src/Protobuf/ProtobufSpec.v
@@ -52,11 +52,11 @@ Local Arguments NToWord : simpl never.
 Local Arguments wordToN : simpl never.
 Local Arguments pow2 : simpl never.
 Local Arguments weqb : simpl never.
-Arguments split1 : simpl never.
-Arguments split2 : simpl never.
-Arguments combine : simpl never.
-Arguments format_wordLE : simpl never.
-Arguments decode_wordLE : simpl never.
+Local Arguments split1 : simpl never.
+Local Arguments split2 : simpl never.
+Local Arguments combine : simpl never.
+Local Arguments format_wordLE : simpl never.
+Local Arguments decode_wordLE : simpl never.
 Local Arguments N.shiftl : simpl never.
 Local Arguments N.shiftr : simpl never.
 Local Arguments N.lor : simpl never.
@@ -84,6 +84,7 @@ Definition PB_WireType_denote (wty : PB_WireType) : Type :=
   | PB_LengthDelimited => list char
   end.
 
+(* Other wire types are deprecated. *)
 Definition PB_WireType_val (wty : PB_WireType) : N :=
   match wty with
   | PB_Varint => 0
@@ -92,6 +93,7 @@ Definition PB_WireType_val (wty : PB_WireType) : N :=
   | PB_LengthDelimited => 2
   end.
 
+(* Convert a number back to wire type. *)
 Definition PB_WireType_val_inv (n : N)
   : PB_WireType + {forall wty, PB_WireType_val wty <> n}.
 Proof.
@@ -121,12 +123,14 @@ Proof.
   end.
 Qed.
 
+(* The value of wire type can fit into 3 bits.  *)
 Theorem PB_WireType_val_3bits (wty : PB_WireType)
   : N.lt (N.log2 (PB_WireType_val wty)) 3%N.
 Proof.
   destruct wty; easy.
 Qed.
 
+(* Default value for wire type. *)
 Definition PB_WireType_default (wty : PB_WireType) : PB_WireType_denote wty :=
   match wty with
   | PB_Varint => 0%N
@@ -135,6 +139,7 @@ Definition PB_WireType_default (wty : PB_WireType) : PB_WireType_denote wty :=
   | PB_LengthDelimited => []
   end.
 
+(* Format a single value. *)
 Definition PB_WireType_format (wty : PB_WireType)
   : FormatM (PB_WireType_denote wty) ByteString :=
   match wty with
@@ -144,47 +149,7 @@ Definition PB_WireType_format (wty : PB_WireType)
   | PB_LengthDelimited => PB_LengthDelimited_format format_word
   end.
 
-Definition PB_WireType_decoder
-           (wty : PB_WireType)
-  : { decode : _ |
-      forall {P : CacheDecode -> Prop}
-        (P_OK : cache_inv_Property P (fun P => forall b cd, P cd -> P (addD cd b))),
-        CorrectDecoder _
-                       (fun _ => True)
-                       (fun _ _ => True)
-                       (PB_WireType_format wty) decode P }.
-Proof.
-  let d := fill_ind_h
-             (PB_WireType_rect
-                (fun pty => DecodeM (PB_WireType_denote pty)
-                                 ByteString)) in
-  refine (exist _ (d wty) _).
-
-  intros; destruct wty; simpl;
-    repeat decode_step idtac.
-  apply Varint_decode_correct; repeat decode_step idtac.
-  apply decode_wordLE_correct; repeat decode_step idtac.
-  apply decode_wordLE_correct; repeat decode_step idtac.
-  eapply shrink_format_correct_True; eauto.
-  apply PB_LengthDelimited_decode_correct; repeat decode_step idtac.
-  apply word_format_sz_eq. intros. eapply word_format_byte; eauto; eauto.
-  intros. apply format_word_some in H; omega.
-  intuition. intros. apply SizedList_predicate_rest_True.
-Defined.
-
-Definition PB_WireType_decode (wty : PB_WireType) :=
-  Eval simpl in proj1_sig (PB_WireType_decoder wty).
-
-Theorem PB_WireType_decode_correct (wty : PB_WireType)
-        {P : CacheDecode -> Prop}
-        (P_OK : cache_inv_Property P (fun P => forall b cd, P cd -> P (addD cd b)))
-  : CorrectDecoder
-      _ (fun _ => True) (fun _ _ => True)
-      (PB_WireType_format wty) (PB_WireType_decode wty) P.
-Proof.
-  apply (proj2_sig (PB_WireType_decoder wty)). auto.
-Qed.
-
+(* A value is always formatted into binary string of the same size. *)
 Theorem PB_WireType_format_sz_eq (wty : PB_WireType)
   : forall d b1 b2 ce1 ce1' ce2 ce2',
     PB_WireType_format wty d ce1 ↝ (b1, ce1') ->
@@ -200,6 +165,7 @@ Proof.
   eapply word_format_sz_eq; eauto.
 Qed.
 
+(* The formatted binary string is byte-aligned. *)
 Theorem PB_WireType_format_byte (wty : PB_WireType)
   : forall d b ce ce',
     PB_WireType_format wty d ce ↝ (b, ce') ->
@@ -214,6 +180,7 @@ Proof.
   intros. eapply word_format_byte; eauto; eauto.
 Qed.
 
+(* A value can never be formatted into empty string *)
 Theorem PB_WireType_format_some (wty : PB_WireType)
   : forall d ce b ce',
     PB_WireType_format wty d ce ↝ (b, ce') ->
@@ -227,50 +194,40 @@ Proof.
   apply PB_LengthDelimited_format_some in H; eauto.
 Qed.
 
-Theorem PB_WireType_decode_lt (wty : PB_WireType)
-  : forall (b : ByteString) (cd : CacheDecode) (d : PB_WireType_denote wty)
-      (b' : ByteString) (cd' : CacheDecode),
-    PB_WireType_decode wty b cd = Some (d, b', cd') -> lt_B b' b.
-Proof.
-  intros. destruct wty; simpl in *.
-  eapply Varint_decode_lt; eauto.
-  eapply decode_wordLE_lt; eauto.
-  eapply decode_wordLE_lt; eauto.
-  eapply PB_LengthDelimited_decode_lt; eauto.
-  eapply decode_word_lt; eauto.
-Qed.
-
-Inductive PB_PrimitiveType : Set :=
-| PB_fixed32 : PB_PrimitiveType
-| PB_fixed64 : PB_PrimitiveType
-| PB_int32 : PB_PrimitiveType
-| PB_int64 : PB_PrimitiveType
-(* | PB_sfixed32 : PB_PrimitiveType *)
-(* | PB_sfixed64 : PB_PrimitiveType *)
-(* | PB_bool : PB_PrimitiveType *)
-| PB_string : PB_PrimitiveType
+Inductive PB_BaseType : Set :=
+| PB_fixed32 : PB_BaseType
+| PB_fixed64 : PB_BaseType
+| PB_int32 : PB_BaseType
+| PB_int64 : PB_BaseType
+| PB_bool : PB_BaseType
+| PB_string : PB_BaseType
 .
 
-Definition PB_PrimitiveType_toWireType (pty : PB_PrimitiveType) : PB_WireType :=
+(* Any base type is encoded as one of the wire type. *)
+Definition PB_BaseType_toWireType (pty : PB_BaseType) : PB_WireType :=
   match pty with
   | PB_fixed32 => PB_32bit
   | PB_fixed64 => PB_64bit
   | PB_int32 => PB_Varint
   | PB_int64 => PB_Varint
+  | PB_bool => PB_Varint
   | PB_string => PB_LengthDelimited
   end.
 
-Definition PB_PrimitiveType_denote (pty : PB_PrimitiveType) : Type :=
-  PB_WireType_denote (PB_PrimitiveType_toWireType pty).
-Arguments PB_PrimitiveType_denote /.
+(* Low-level denotation for base type. *)
+Definition PB_BaseType_denote (pty : PB_BaseType) : Type :=
+  PB_WireType_denote (PB_BaseType_toWireType pty).
+Arguments PB_BaseType_denote /.
 
-Definition PB_PrimitiveType_default (pty : PB_PrimitiveType) : PB_PrimitiveType_denote pty :=
-  PB_WireType_default (PB_PrimitiveType_toWireType pty).
-Arguments PB_PrimitiveType_default /.
+(* Default value for base type. *)
+Definition PB_BaseType_default (pty : PB_BaseType) : PB_BaseType_denote pty :=
+  PB_WireType_default (PB_BaseType_toWireType pty).
+Arguments PB_BaseType_default /.
 
+(* The mutually inductive definition for Descriptor, Field, Protobuf Type and Base type. *)
 Inductive PB_SingularType : Set :=
-| PB_Primitive : PB_PrimitiveType -> PB_SingularType
-| PB_Embedded : PB_Message -> PB_SingularType
+| PB_Base : PB_BaseType -> PB_SingularType
+| PB_Embedded : PB_Descriptor -> PB_SingularType
 
 with PB_Type : Set :=
      | PB_Singular : PB_SingularType -> PB_Type
@@ -279,30 +236,31 @@ with PB_Type : Set :=
 with PB_Field : Set :=
      | Build_PB_Field : PB_Type -> string -> N -> PB_Field
 
-with PB_Message : Set :=
-     | Build_PB_Message : forall {n}, Vector.t PB_Field n -> PB_Message.
+with PB_Descriptor : Set :=
+     | Build_PB_Descriptor : forall {n}, Vector.t PB_Field n -> PB_Descriptor.
 
+(* Mutual induction principle. *)
 Scheme PB_SingularType_mut := Induction for PB_SingularType Sort Prop
   with PB_Type_mut := Induction for PB_Type Sort Prop
   with PB_Field_mut := Induction for PB_Field Sort Prop
-  with PB_Message_mut := Induction for PB_Message Sort Prop.
+  with PB_Descriptor_mut := Induction for PB_Descriptor Sort Prop.
 
-Section PB_Message_induction.
+Section PB_Descriptor_induction.
   Variable P_sty : PB_SingularType -> Prop.
   Variable P_ty : PB_Type -> Prop.
   Variable P_fld : PB_Field -> Prop.
-  Variable P_desc : PB_Message -> Prop.
-  Variable f0 : forall pty : PB_PrimitiveType, P_sty (PB_Primitive pty).
-  Variable f1 : forall desc : PB_Message, P_desc desc -> P_sty (PB_Embedded desc).
+  Variable P_desc : PB_Descriptor -> Prop.
+  Variable f0 : forall pty : PB_BaseType, P_sty (PB_Base pty).
+  Variable f1 : forall desc : PB_Descriptor, P_desc desc -> P_sty (PB_Embedded desc).
   Variable f2 : forall sty : PB_SingularType, P_sty sty -> P_ty (PB_Singular sty).
   Variable f3 : forall sty : PB_SingularType, P_sty sty -> P_ty (PB_Repeated sty).
   Variable f4 : forall ty : PB_Type, P_ty ty -> forall (s : string) (n : N), P_fld (Build_PB_Field ty s n).
-  Variable f5 : forall (n : nat) (v : Vector.t PB_Field n), Vector.Forall P_fld v -> P_desc (Build_PB_Message v).
+  Variable f5 : forall (n : nat) (v : Vector.t PB_Field n), Vector.Forall P_fld v -> P_desc (Build_PB_Descriptor v).
 
   Fixpoint PB_SingularType_ind' (sty : PB_SingularType) : P_sty sty
   with PB_Type_ind' (ty : PB_Type) : P_ty ty
   with PB_Field_ind' (fld : PB_Field) : P_fld fld
-  with PB_Message_ind' (desc : PB_Message) : P_desc desc.
+  with PB_Descriptor_ind' (desc : PB_Descriptor) : P_desc desc.
   Proof.
     destruct sty. apply f0. apply f1. auto.
     destruct ty. apply f2. auto. apply f3. auto.
@@ -311,25 +269,38 @@ Section PB_Message_induction.
     induction desc; constructor; auto.
   Defined.
 
-End PB_Message_induction.
+End PB_Descriptor_induction.
 
+(* Handy helper functions for accessing the projections.. *)
 Definition PB_FieldType (fld : PB_Field) := let (ty, _, _) := fld in ty.
 Definition PB_FieldName (fld : PB_Field) := let (_, name, _) := fld in name.
 Definition PB_FieldTag (fld : PB_Field) := let (_, _, tag) := fld in tag.
 
 Definition PB_Desc := Vector.t PB_Field.
 
-Definition PB_MessageLen (desc : PB_Message) :=
+Definition PB_DescriptorLen (desc : PB_Descriptor) :=
   let (n, _) := desc in n.
 
-Definition PB_MessageDesc (desc : PB_Message) :=
-  let (_, v) return (Vector.t _ (PB_MessageLen desc)) := desc in v.
+Definition PB_DescriptorDesc (desc : PB_Descriptor) :=
+  let (_, v) return (Vector.t _ (PB_DescriptorLen desc)) := desc in v.
 
-Definition PB_Message_tags' {n} (desc : PB_Desc n) :=
+(* Get the list of tags from the descriptor. *)
+Definition PB_Descriptor_tags' {n} (desc : PB_Desc n) :=
   Vector.map PB_FieldTag desc.
 
-Definition PB_Message_tags (desc : PB_Message) :=
-  PB_Message_tags' (PB_MessageDesc desc).
+Definition PB_Descriptor_tags (desc : PB_Descriptor) :=
+  PB_Descriptor_tags' (PB_DescriptorDesc desc).
+
+(* Sanity check for tags function. *)
+Lemma PB_Descriptor_tags_correct (desc : PB_Descriptor)
+  : forall i, Vector.nth (PB_Descriptor_tags desc) i
+         = PB_FieldTag (Vector.nth (PB_DescriptorDesc desc) i).
+Proof.
+  destruct desc as [n desc]. simpl in *.
+  unfold PB_Descriptor_tags. simpl.
+  intros. apply Vector.nth_map. reflexivity.
+Qed.
+
 
 Definition vec_eq_dec
            {A} (A_eq_dec : forall (a1 a2 : A), {a1 = a2} + {a1 <> a2})
@@ -351,13 +322,14 @@ Proof.
   }
 Defined.
 
+(* Equality of Descriptor is decidable. *)
 Fixpoint PB_SingularType_eq_dec (sty1 sty2 : PB_SingularType)
   : {sty1 = sty2} + {sty1 <> sty2}
 with PB_Type_eq_dec (ty1 ty2 : PB_Type)
      : {ty1 = ty2} + {ty1 <> ty2}
 with PB_Field_eq_dec (fld1 fld2 : PB_Field)
      : {fld1 = fld2} + {fld1 <> fld2}
-with PB_Message_eq_dec (desc1 desc2 : PB_Message)
+with PB_Descriptor_eq_dec (desc1 desc2 : PB_Descriptor)
   : {desc1 = desc2} + {desc1 <> desc2}.
 Proof.
   all : repeat decide equality.
@@ -367,7 +339,7 @@ Proof.
     assert ({desc1 = desc2} + {desc1 <> desc2}) as L. {
       apply vec_eq_dec. auto.
     }
-    clear PB_Message_eq_dec.
+    clear PB_Descriptor_eq_dec.
     destruct L.
     - left. subst. reflexivity.
     - right. inversion 1.
@@ -377,83 +349,77 @@ Proof.
   }
 Defined.
 
-Definition PB_Message_heading' denote (desc : PB_Message) :=
-  BuildHeading (Vector.map denote (PB_MessageDesc desc)).
-Arguments PB_Message_heading' /.
+(* The low-level denotation of Descriptors, Fields, Protobuf type and Base type.
+   We use the Tuple type in Fiat, which is essentially a heterogeneous list,
+   supporting bounded element access. *)
+Definition PB_Descriptor_heading' denote (desc : PB_Descriptor) :=
+  BuildHeading (Vector.map denote (PB_DescriptorDesc desc)).
+Arguments PB_Descriptor_heading' /.
 
 Fixpoint PB_Type_denote (ty : PB_Type) : Type :=
   match ty with
   | PB_Singular sty =>
     match sty with
-    | PB_Primitive pty => PB_PrimitiveType_denote pty
-    | PB_Embedded desc => option (PB_Message_denote desc)
+    | PB_Base pty => PB_BaseType_denote pty
+    | PB_Embedded desc => option (PB_Descriptor_denote desc)
     end
   | PB_Repeated sty =>
     match sty with
-    | PB_Primitive pty => list (PB_PrimitiveType_denote pty)
-    | PB_Embedded desc => list (PB_Message_denote desc)
+    | PB_Base pty => list (PB_BaseType_denote pty)
+    | PB_Embedded desc => list (PB_Descriptor_denote desc)
     end
   end
 
 with PB_Field_denote (fld : PB_Field) : Attribute :=
        ((PB_FieldName fld) :: PB_Type_denote (PB_FieldType fld))%Attribute
 
-with PB_Message_denote (desc : PB_Message) : Type :=
-       @Tuple (PB_Message_heading' PB_Field_denote desc).
+with PB_Descriptor_denote (desc : PB_Descriptor) : Type :=
+       @Tuple (PB_Descriptor_heading' PB_Field_denote desc).
 
-Definition PB_Message_heading := PB_Message_heading' PB_Field_denote.
+Definition PB_Descriptor_heading := PB_Descriptor_heading' PB_Field_denote.
 
+(* The default value of descriptor. *)
 Definition PB_Type_default (ty : PB_Type) : PB_Type_denote ty :=
   match ty with
   | PB_Singular sty =>
     match sty with
-    | PB_Primitive pty => PB_PrimitiveType_default pty
+    | PB_Base pty => PB_BaseType_default pty
     | PB_Embedded _ => None
     end
   | PB_Repeated sty =>
     match sty with
-    | PB_Primitive _ => nil
+    | PB_Base _ => nil
     | PB_Embedded _ => nil
     end
   end.
 
-Fixpoint PB_Message_default' {n} (desc : PB_Desc n) : PB_Message_denote (Build_PB_Message desc).
+Fixpoint PB_Descriptor_default' {n} (desc : PB_Desc n) : PB_Descriptor_denote (Build_PB_Descriptor desc).
 Proof.
   refine
-    (match desc return (PB_Message_denote (Build_PB_Message desc)) with
+    (match desc return (PB_Descriptor_denote (Build_PB_Descriptor desc)) with
      | Vector.nil => inil2 (B:=id)
      | Vector.cons fld _ desc' =>
-       icons2 (B:=id) _ (PB_Message_default' _ desc')
+       icons2 (B:=id) _ (PB_Descriptor_default' _ desc')
      end).
   destruct fld as [ty ? ?].
   exact (PB_Type_default ty).
 Defined.
 
-Definition PB_Message_default (desc : PB_Message) : PB_Message_denote desc :=
+Definition PB_Descriptor_default (desc : PB_Descriptor) : PB_Descriptor_denote desc :=
   match desc with
-  | Build_PB_Message _ desc => PB_Message_default' desc
+  | Build_PB_Descriptor _ desc => PB_Descriptor_default' desc
   end.
 
-(* :TODO: show equivalence of two default functions. *)
-Definition PB_Message_default2 (desc : PB_Message) := PB_Message_default' (PB_MessageDesc desc).
-
-Lemma PB_Message_tags_correct (desc : PB_Message)
-  : forall i, Vector.nth (PB_Message_tags desc) i
-         = PB_FieldTag (Vector.nth (PB_MessageDesc desc) i).
-Proof.
-  destruct desc as [n desc]. simpl in *.
-  unfold PB_Message_tags. simpl.
-  intros. apply Vector.nth_map. reflexivity.
-Qed.
-
+(* Tag has to be in a range by the specification, although it is not important
+   for our implementation. *)
 Definition PB_FieldTag_OK (t : N) :=
   ((1 <= t <= 18999) \/ (20000 <= t <= 536870911))%N.
 
-(* TODO: This should probably be synthesized automatically. *)
+(* Decision procedure for checking tag. *)
+(* TODO: use Decidable module to synthesize it. *)
 Definition PB_FieldTag_OK_dec (t : N) :=
   (((N.leb 1 t) && (N.leb t 18999)) || ((N.leb 20000 t) && (N.leb t 536870911)))%bool.
 
-(* Should use reflect here. *)
 Definition PB_FieldTag_OK_true_iff (t : N)
   : PB_FieldTag_OK_dec t = true <-> (PB_FieldTag_OK t).
 Proof.
@@ -466,7 +432,6 @@ Proof.
     end.
 Qed.
 
-(* Need abstraction. *)
 Definition PB_FieldTag_OK_false_iff (t : N)
   : PB_FieldTag_OK_dec t = false <-> ~ (PB_FieldTag_OK t).
 Proof.
@@ -475,6 +440,7 @@ Proof.
   apply PB_FieldTag_OK_true_iff in Heqb. congruence.
 Qed.
 
+(* Field name can not be empty. *)
 Definition PB_FieldName_OK (n : string) :=
   n <> EmptyString.
 
@@ -482,10 +448,39 @@ Definition PB_Field_OK (fld : PB_Field) :=
   PB_FieldName_OK (PB_FieldName fld) /\
   PB_FieldTag_OK (PB_FieldTag fld).
 
-Definition PB_Message_tags_nodup (desc : PB_Message) :=
-  forall i1 i2 : Fin.t (PB_MessageLen desc),
-    Vector.nth (PB_Message_tags desc) i1 = Vector.nth (PB_Message_tags desc) i2 ->
+(* Tags are unique. *)
+Definition PB_Descriptor_tags_nodup (desc : PB_Descriptor) :=
+  forall i1 i2 : Fin.t (PB_DescriptorLen desc),
+    Vector.nth (PB_Descriptor_tags desc) i1 = Vector.nth (PB_Descriptor_tags desc) i2 ->
     i1 = i2.
+
+(* Names are unique. *)
+Definition PB_Descriptor_names_nodup (desc : PB_Descriptor) :=
+  forall i1 i2 : Fin.t (PB_DescriptorLen desc),
+    Vector.nth (Vector.map PB_FieldName (PB_DescriptorDesc desc)) i1 = Vector.nth (Vector.map PB_FieldName (PB_DescriptorDesc desc)) i2 ->
+    i1 = i2.
+
+(* Predicate for valid descriptor. *)
+Fixpoint PB_Descriptor_OK (desc : PB_Descriptor) : Prop :=
+  Vector.Forall PB_Field_OK (PB_DescriptorDesc desc) /\
+  PB_Descriptor_tags_nodup desc /\ PB_Descriptor_names_nodup desc /\
+  match desc with
+  | Build_PB_Descriptor n desc =>
+    (fix OK {n} (desc : PB_Desc n) :=
+       match desc with
+       | Vector.nil => True
+       | Vector.cons h _ t =>
+         match h with
+         | Build_PB_Field ty _ _ =>
+           match ty with
+           | PB_Singular (PB_Embedded desc'')
+           | PB_Repeated (PB_Embedded desc'') =>
+             PB_Descriptor_OK desc''
+           | _ => True
+           end
+         end /\ OK t
+       end) n desc
+  end.
 
 Lemma vec_nodup_cons {A n} (h : A) (v : Vector.t A n)
   : (forall i1 i2 : Fin.t (S n), Vector.nth (Vector.cons _ h _ v) i1 = Vector.nth (Vector.cons _ h _ v) i2 -> i1 = i2) ->
@@ -498,38 +493,13 @@ Proof.
   simpl in H. apply H in H0. inversion H0. existT_eq_dec. easy.
 Qed.
 
-Definition PB_Message_names_nodup (desc : PB_Message) :=
-  forall i1 i2 : Fin.t (PB_MessageLen desc),
-    Vector.nth (Vector.map PB_FieldName (PB_MessageDesc desc)) i1 = Vector.nth (Vector.map PB_FieldName (PB_MessageDesc desc)) i2 ->
-    i1 = i2.
-
-Fixpoint PB_Message_OK (desc : PB_Message) : Prop :=
-  Vector.Forall PB_Field_OK (PB_MessageDesc desc) /\
-  PB_Message_tags_nodup desc /\ PB_Message_names_nodup desc /\
-  match desc with
-  | Build_PB_Message n desc =>
-    (fix OK {n} (desc : PB_Desc n) :=
-       match desc with
-       | Vector.nil => True
-       | Vector.cons h _ t =>
-         match h with
-         | Build_PB_Field ty _ _ =>
-           match ty with
-           | PB_Singular (PB_Embedded desc'')
-           | PB_Repeated (PB_Embedded desc'') =>
-             PB_Message_OK desc''
-           | _ => True
-           end
-         end /\ OK t
-       end) n desc
-  end.
-
-Theorem PB_Message_OK_sub (desc : PB_Message)
-  : PB_Message_OK desc ->
-    forall fld, Vector.In fld (PB_MessageDesc desc) ->
+(* Descriptor is valid implies all of its embedded descriptors are valid. *)
+Theorem PB_Descriptor_OK_sub (desc : PB_Descriptor)
+  : PB_Descriptor_OK desc ->
+    forall fld, Vector.In fld (PB_DescriptorDesc desc) ->
            forall desc', (PB_FieldType fld = PB_Singular (PB_Embedded desc') \/
                      PB_FieldType fld = PB_Repeated (PB_Embedded desc')) ->
-                    PB_Message_OK desc'.
+                    PB_Descriptor_OK desc'.
 Proof.
   destruct desc as [n desc]. simpl.
   intros. induction H0.
@@ -537,13 +507,13 @@ Proof.
   - apply IHIn. destruct H as [? [? [? [? ?]]]].
     repeat split; auto.
     + inversion H. existT_eq_dec. congruence.
-    + unfold PB_Message_tags_nodup in *. eapply vec_nodup_cons. simpl in *. eauto.
-    + unfold PB_Message_names_nodup in *. eapply vec_nodup_cons. simpl in *. eauto.
+    + unfold PB_Descriptor_tags_nodup in *. eapply vec_nodup_cons. simpl in *. eauto.
+    + unfold PB_Descriptor_names_nodup in *. eapply vec_nodup_cons. simpl in *. eauto.
 Qed.
 
-Lemma PB_denote_type_eq (desc : PB_Message) (i : Fin.t (PB_MessageLen desc))
-  : PB_Type_denote (PB_FieldType (Vector.nth (PB_MessageDesc desc) i))
-    = Domain (PB_Message_heading desc) i.
+Lemma PB_denote_type_eq (desc : PB_Descriptor) (i : Fin.t (PB_DescriptorLen desc))
+  : PB_Type_denote (PB_FieldType (Vector.nth (PB_DescriptorDesc desc) i))
+    = Domain (PB_Descriptor_heading desc) i.
 Proof.
   destruct desc as [n desc]. simpl in *.
   induction desc; intros.
@@ -554,11 +524,12 @@ Proof.
     + apply IHdesc.
 Defined.
 
-Lemma PB_Message_default_correct (desc : PB_Message)
-  : forall (i : Fin.t (PB_MessageLen desc)),
+(* Sanity check for default function *)
+Lemma PB_Descriptor_default_correct (desc : PB_Descriptor)
+  : forall (i : Fin.t (PB_DescriptorLen desc)),
     type_cast (PB_denote_type_eq desc i)
-              (PB_Type_default (PB_FieldType (Vector.nth (PB_MessageDesc desc) i)))
-    = ith2 (PB_Message_default2 desc) i.
+              (PB_Type_default (PB_FieldType (Vector.nth (PB_DescriptorDesc desc) i)))
+    = ith2 (PB_Descriptor_default' (PB_DescriptorDesc desc)) i.
 Proof.
   destruct desc as [n desc]. simpl in *.
   induction desc; intros.
@@ -569,8 +540,9 @@ Proof.
     + apply IHdesc.
 Qed.
 
-Definition BoundedTag (desc : PB_Message) :=
-  BoundedIndex (PB_Message_tags desc).
+(* A bounded tag is a tag which must be in the descriptor. *)
+Definition BoundedTag (desc : PB_Descriptor) :=
+  BoundedIndex (PB_Descriptor_tags desc).
 
 Record UnboundedIndex {A} {n : nat} (Bound : Vector.t A n) :=
   { uindex : A;
@@ -579,15 +551,17 @@ Record UnboundedIndex {A} {n : nat} (Bound : Vector.t A n) :=
 
 Global Arguments uindex {A n Bound} u.
 
-Definition UnboundedTag (desc : PB_Message) :=
-  UnboundedIndex (PB_Message_tags desc).
+(* An unbounded tag is a tag which must not be in the descriptor. *)
+Definition UnboundedTag (desc : PB_Descriptor) :=
+  UnboundedIndex (PB_Descriptor_tags desc).
 
-Theorem BoundedTag_inj (desc : PB_Message)
-  : PB_Message_OK desc ->
+(* Two bounded tags are equal if their tag numbers are equal. *)
+Theorem BoundedTag_inj (desc : PB_Descriptor)
+  : PB_Descriptor_OK desc ->
     forall t1 t2 : BoundedTag desc,
       bindex t1 = bindex t2 -> t1 = t2.
 Proof.
-  unfold PB_Message_OK, PB_Message_tags_nodup.
+  unfold PB_Descriptor_OK, PB_Descriptor_tags_nodup.
   destruct desc as [n desc].
   intros [_ [? _]]; intros. destruct t1, t2. destruct indexb, indexb0.
   simpl in *. subst. apply H in H0. subst. reflexivity.
@@ -602,21 +576,22 @@ Proof.
     auto.
 Qed.
 
-Theorem PB_Field_inj (desc : PB_Message)
-  : PB_Message_OK desc ->
+(* Two fields are equal if their tags are equal. *)
+Theorem PB_Field_inj (desc : PB_Descriptor)
+  : PB_Descriptor_OK desc ->
     forall fld1 fld2 : PB_Field,
-      Vector.In fld1 (PB_MessageDesc desc) -> Vector.In fld2 (PB_MessageDesc desc) ->
+      Vector.In fld1 (PB_DescriptorDesc desc) -> Vector.In fld2 (PB_DescriptorDesc desc) ->
       PB_FieldTag fld1 = PB_FieldTag fld2 ->
       fld1 = fld2.
 Proof.
-  unfold PB_Message_OK, PB_Message_tags_nodup.
+  unfold PB_Descriptor_OK, PB_Descriptor_tags_nodup.
   destruct desc as [n desc].
   intros [_ [? _]]; intros.
   destruct (vector_in_fin _ _ H0).
   destruct (vector_in_fin _ _ H1).
   subst.
   f_equal. apply H.
-  rewrite !PB_Message_tags_correct.
+  rewrite !PB_Descriptor_tags_correct.
   assumption.
 Qed.
 
@@ -630,21 +605,23 @@ Proof.
     intros. simpl in *. constructor. apply IHi.
 Qed.
 
-Theorem BoundedTag_in (desc : PB_Message)
-  : forall t1 : BoundedTag desc, Vector.In (bindex t1) (PB_Message_tags desc).
+(* Some immediate lemmas for bounded and unbounded tags. *)
+Lemma BoundedTag_in (desc : PB_Descriptor)
+  : forall t1 : BoundedTag desc, Vector.In (bindex t1) (PB_Descriptor_tags desc).
 Proof.
   intros. destruct t1. destruct indexb. simpl in *.
   subst. eapply vector_in; eauto.
 Qed.
 
-Theorem BoundedTag_not_unbounded (desc : PB_Message)
+Lemma BoundedTag_not_unbounded (desc : PB_Descriptor)
   : forall (t1 : BoundedTag desc) (t2 : UnboundedTag desc), bindex t1 <> uindex t2.
 Proof.
   intros. intro. pose proof (BoundedTag_in _ t1). destruct t2. simpl in *.
   subst. easy.
 Qed.
 
-Fixpoint PB_Message_boundedTag' {n} (tags : Vector.t N n) (m : N)
+(* A decision procedure to convert a tag number to bounded or unbounded tag. *)
+Fixpoint PB_Descriptor_boundedTag' {n} (tags : Vector.t N n) (m : N)
   : {ibound : _ | Vector.nth tags ibound = m} + {~ Vector.In m tags}.
 Proof.
   refine
@@ -654,7 +631,7 @@ Proof.
        if N.eq_dec t m then
          inleft (exist _ Fin.F1 _)
        else
-         match PB_Message_boundedTag' n' tags' m with
+         match PB_Descriptor_boundedTag' n' tags' m with
          | inleft (exist i _) =>
            inleft (exist _ (Fin.FS i) _)
          | inright _ => inright _
@@ -666,78 +643,80 @@ Proof.
        subst; congruence).
 Defined.
 
-Definition PB_Message_boundedTag (desc : PB_Message) (m : N)
+Definition PB_Descriptor_boundedTag (desc : PB_Descriptor) (m : N)
   : (BoundedTag desc) + (UnboundedTag desc) :=
-  match PB_Message_boundedTag' (PB_Message_tags desc) m with
+  match PB_Descriptor_boundedTag' (PB_Descriptor_tags desc) m with
   | inleft (exist i pf) => inl {| bindex := m; indexb := {| ibound := i; boundi := pf |} |}
   | inright pf => inr {| uindex := m; uboundi := pf |}
   end.
 
-Theorem PB_Message_boundedTag_correct (desc : PB_Message) (m : N)
-  : forall tag, PB_Message_boundedTag desc m = inl tag -> bindex tag = m.
+(* Sanity check and useful lemmas for later proofs. *)
+Lemma PB_Descriptor_boundedTag_correct (desc : PB_Descriptor) (m : N)
+  : forall tag, PB_Descriptor_boundedTag desc m = inl tag -> bindex tag = m.
 Proof.
-  unfold PB_Message_boundedTag.
-  intros. destruct PB_Message_boundedTag'; try easy.
+  unfold PB_Descriptor_boundedTag.
+  intros. destruct PB_Descriptor_boundedTag'; try easy.
   destruct s. inversion H. reflexivity.
 Qed.
 
-Theorem PB_Message_boundedTag_correct' (desc : PB_Message) (m : N)
-  : forall tag, PB_Message_boundedTag desc m = inr tag -> uindex tag = m.
+Lemma PB_Descriptor_boundedTag_correct' (desc : PB_Descriptor) (m : N)
+  : forall tag, PB_Descriptor_boundedTag desc m = inr tag -> uindex tag = m.
 Proof.
-  unfold PB_Message_boundedTag.
-  intros. destruct PB_Message_boundedTag'. destruct s.
+  unfold PB_Descriptor_boundedTag.
+  intros. destruct PB_Descriptor_boundedTag'. destruct s.
   easy. inversion H. reflexivity.
 Qed.
 
-Theorem PB_Message_boundedTag_inv (desc : PB_Message)
-  : PB_Message_OK desc -> forall tag, PB_Message_boundedTag desc (bindex tag) = inl tag.
+Lemma PB_Descriptor_boundedTag_inv (desc : PB_Descriptor)
+  : PB_Descriptor_OK desc -> forall tag, PB_Descriptor_boundedTag desc (bindex tag) = inl tag.
 Proof.
-  intros. destruct (PB_Message_boundedTag desc (bindex tag)) eqn:?.
-  apply PB_Message_boundedTag_correct in Heqs.
+  intros. destruct (PB_Descriptor_boundedTag desc (bindex tag)) eqn:?.
+  apply PB_Descriptor_boundedTag_correct in Heqs.
   apply BoundedTag_inj in Heqs; eauto. subst. auto.
-  exfalso. apply PB_Message_boundedTag_correct' in Heqs.
+  exfalso. apply PB_Descriptor_boundedTag_correct' in Heqs.
   destruct tag as [? [? ?]]. destruct u. simpl in *.
   subst. apply uboundi0. apply vector_in.
 Qed.
 
-Theorem PB_Message_boundedTag_notr (desc : PB_Message)
-  : PB_Message_OK desc -> forall (tag : BoundedTag desc) utag, PB_Message_boundedTag desc (bindex tag) <> inr utag.
+Lemma PB_Descriptor_boundedTag_notr (desc : PB_Descriptor)
+  : PB_Descriptor_OK desc -> forall (tag : BoundedTag desc) utag, PB_Descriptor_boundedTag desc (bindex tag) <> inr utag.
 Proof.
-  intros. intro. apply PB_Message_boundedTag_correct' in H0.
+  intros. intro. apply PB_Descriptor_boundedTag_correct' in H0.
   destruct desc. destruct tag as [? [? ?]]; destruct utag. simpl in *. subst.
   apply uboundi0. apply vector_in.
 Qed.
 
-Theorem PB_Message_boundedTag_notl (desc : PB_Message)
-  : PB_Message_OK desc -> forall (utag : UnboundedTag desc) tag, PB_Message_boundedTag desc (uindex utag) <> inl tag.
+Lemma PB_Descriptor_boundedTag_notl (desc : PB_Descriptor)
+  : PB_Descriptor_OK desc -> forall (utag : UnboundedTag desc) tag, PB_Descriptor_boundedTag desc (uindex utag) <> inl tag.
 Proof.
-  intros. intro. apply PB_Message_boundedTag_correct in H0.
+  intros. intro. apply PB_Descriptor_boundedTag_correct in H0.
   destruct desc. destruct tag as [? [? ?]]; destruct utag. simpl in *. subst.
   apply uboundi0. apply vector_in.
 Qed.
 
-Definition PB_Message_tagToIndex {desc : PB_Message}
+(* Map a bounded tag to its index of the descriptor vector. *)
+Definition PB_Descriptor_tagToIndex {desc : PB_Descriptor}
          (tag : BoundedTag desc) :=
   ibound (indexb tag).
-Arguments PB_Message_tagToIndex /.
+Arguments PB_Descriptor_tagToIndex /.
 
-Theorem PB_Message_tagToIndex_correct (desc : PB_Message)
+Lemma PB_Descriptor_tagToIndex_correct (desc : PB_Descriptor)
         (tag : BoundedTag desc)
-  : PB_FieldTag (Vector.nth (PB_MessageDesc desc) (PB_Message_tagToIndex tag))
+  : PB_FieldTag (Vector.nth (PB_DescriptorDesc desc) (PB_Descriptor_tagToIndex tag))
     = bindex tag.
 Proof.
   destruct desc as [n desc].
-  rewrite <- PB_Message_tags_correct.
+  rewrite <- PB_Descriptor_tags_correct.
   destruct tag. destruct indexb.
   eauto.
 Qed.
 
-Theorem PB_Message_tagToIndex_correct' (desc : PB_Message)
+Lemma PB_Descriptor_tagToIndex_correct' (desc : PB_Descriptor)
         (tag : BoundedTag desc)
-  : PB_Message_OK desc ->
-    forall fld, Vector.In fld (PB_MessageDesc desc) ->
+  : PB_Descriptor_OK desc ->
+    forall fld, Vector.In fld (PB_DescriptorDesc desc) ->
            PB_FieldTag fld = bindex tag ->
-           fld = Vector.nth (PB_MessageDesc desc) (PB_Message_tagToIndex tag).
+           fld = Vector.nth (PB_DescriptorDesc desc) (PB_Descriptor_tagToIndex tag).
 Proof.
   intros. destruct desc as [n desc].
   destruct tag. destruct indexb.
@@ -747,117 +726,88 @@ Proof.
   apply Fin.caseS; intros.
   - subst. eapply PB_Field_inj; eauto. constructor.
   - eapply PB_Field_inj; eauto; clear H; simpl in *. constructor. apply vector_in.
-    subst. rewrite <- (PB_Message_tags_correct (Build_PB_Message desc)). auto.
+    subst. rewrite <- (PB_Descriptor_tags_correct (Build_PB_Descriptor desc)). auto.
 Qed.
 
-Definition PB_Message_tagToType {desc : PB_Message}
+(* Look up the type of the field by its tag. *)
+Definition PB_Descriptor_tagToType {desc : PB_Descriptor}
            (tag : BoundedTag desc) :=
-  PB_FieldType (Vector.nth (PB_MessageDesc desc) (PB_Message_tagToIndex tag)).
+  PB_FieldType (Vector.nth (PB_DescriptorDesc desc) (PB_Descriptor_tagToIndex tag)).
 
-Theorem PB_Message_tagToType_correct (desc : PB_Message)
+Theorem PB_Descriptor_tagToType_correct (desc : PB_Descriptor)
         (tag : BoundedTag desc)
-  : PB_Message_OK desc ->
-    forall fld, Vector.In fld (PB_MessageDesc desc) ->
+  : PB_Descriptor_OK desc ->
+    forall fld, Vector.In fld (PB_DescriptorDesc desc) ->
            PB_FieldTag fld = bindex tag ->
-           PB_FieldType fld = PB_Message_tagToType tag.
+           PB_FieldType fld = PB_Descriptor_tagToType tag.
 Proof.
   intros.
-  rewrite (PB_Message_tagToIndex_correct' desc tag H fld); eauto.
+  rewrite (PB_Descriptor_tagToIndex_correct' desc tag H fld); eauto.
 Qed.
 
-Theorem PB_Message_OK_sub_tagToType (desc : PB_Message)
-  : PB_Message_OK desc ->
+(* All embedded descriptors of a valid descripto are valid. *)
+Lemma PB_Descriptor_OK_sub_tagToType (desc : PB_Descriptor)
+  : PB_Descriptor_OK desc ->
     forall (tag : BoundedTag desc) desc',
-      (PB_Message_tagToType tag = PB_Singular (PB_Embedded desc') \/
-       PB_Message_tagToType tag = PB_Repeated (PB_Embedded desc')) ->
-      PB_Message_OK desc'.
+      (PB_Descriptor_tagToType tag = PB_Singular (PB_Embedded desc') \/
+       PB_Descriptor_tagToType tag = PB_Repeated (PB_Embedded desc')) ->
+      PB_Descriptor_OK desc'.
 Proof.
-  intros. eapply PB_Message_OK_sub in H; eauto.
+  intros. eapply PB_Descriptor_OK_sub in H; eauto.
   destruct desc as [n desc]. destruct tag as [? [? ?]]. simpl.
   apply vector_in.
 Qed.
 
-Definition PB_Message_tagToDenoteType {desc : PB_Message}
+(* Mainly for type casting. *)
+Definition PB_Descriptor_tagToDenoteType {desc : PB_Descriptor}
            (tag : BoundedTag desc) :=
-  Domain (PB_Message_heading desc) (PB_Message_tagToIndex tag).
+  Domain (PB_Descriptor_heading desc) (PB_Descriptor_tagToIndex tag).
 
-Theorem PB_Message_tagToDenoteType_correct (desc : PB_Message)
+Theorem PB_Descriptor_tagToDenoteType_correct (desc : PB_Descriptor)
         (tag : BoundedTag desc)
-  : PB_Type_denote (PB_Message_tagToType tag)
-    = PB_Message_tagToDenoteType tag.
+  : PB_Type_denote (PB_Descriptor_tagToType tag)
+    = PB_Descriptor_tagToDenoteType tag.
 Proof.
   apply PB_denote_type_eq.
 Defined.
 
-Opaque PB_Message_tagToDenoteType_correct.
+Opaque PB_Descriptor_tagToDenoteType_correct.
 
-Definition PB_Message_lookup' {n} {desc : PB_Desc n}
-           (msg : PB_Message_denote (Build_PB_Message desc))
-           (tag : BoundedTag (Build_PB_Message desc)) :=
-  type_cast_r (PB_Message_tagToDenoteType_correct (Build_PB_Message desc) tag)
-              (GetAttributeRaw msg (PB_Message_tagToIndex tag)).
+(* Look up value of the field of the given message by its tag. *)
+Definition PB_Descriptor_lookup' {n} {desc : PB_Desc n}
+           (msg : PB_Descriptor_denote (Build_PB_Descriptor desc))
+           (tag : BoundedTag (Build_PB_Descriptor desc)) :=
+  type_cast_r (PB_Descriptor_tagToDenoteType_correct (Build_PB_Descriptor desc) tag)
+              (GetAttributeRaw msg (PB_Descriptor_tagToIndex tag)).
 
-Definition PB_Message_lookup {desc : PB_Message} :=
-  match desc return PB_Message_denote desc ->
+Definition PB_Descriptor_lookup {desc : PB_Descriptor} :=
+  match desc return PB_Descriptor_denote desc ->
                     forall tag : BoundedTag desc,
-                      PB_Type_denote (PB_Message_tagToType tag) with
-  | Build_PB_Message _ v =>
-    fun msg tag => @PB_Message_lookup' _ v msg tag
+                      PB_Type_denote (PB_Descriptor_tagToType tag) with
+  | Build_PB_Descriptor _ v =>
+    fun msg tag => @PB_Descriptor_lookup' _ v msg tag
   end.
 
-Definition PB_Message_update' {n} {desc : PB_Desc n}
-           (msg : PB_Message_denote (Build_PB_Message desc))
-           (tag : BoundedTag (Build_PB_Message desc))
-           (value : PB_Type_denote (PB_Message_tagToType tag))
-  : PB_Message_denote (Build_PB_Message desc) :=
-  SetAttributeRaw msg (PB_Message_tagToIndex tag)
+(* Update value of the field of the given message by its tag. *)
+Definition PB_Descriptor_update' {n} {desc : PB_Desc n}
+           (msg : PB_Descriptor_denote (Build_PB_Descriptor desc))
+           (tag : BoundedTag (Build_PB_Descriptor desc))
+           (value : PB_Type_denote (PB_Descriptor_tagToType tag))
+  : PB_Descriptor_denote (Build_PB_Descriptor desc) :=
+  SetAttributeRaw msg (PB_Descriptor_tagToIndex tag)
                   (type_cast
-                     (PB_Message_tagToDenoteType_correct
-                        (Build_PB_Message desc) tag)
+                     (PB_Descriptor_tagToDenoteType_correct
+                        (Build_PB_Descriptor desc) tag)
                      value).
 
-Definition PB_Message_update {desc : PB_Message} :=
-  match desc return PB_Message_denote desc ->
+Definition PB_Descriptor_update {desc : PB_Descriptor} :=
+  match desc return PB_Descriptor_denote desc ->
                     forall tag : BoundedTag desc,
-                      PB_Type_denote (PB_Message_tagToType tag) ->
-                      PB_Message_denote desc with
-  | Build_PB_Message _ v =>
-    fun msg tag value => PB_Message_update' msg tag value
+                      PB_Type_denote (PB_Descriptor_tagToType tag) ->
+                      PB_Descriptor_denote desc with
+  | Build_PB_Descriptor _ v =>
+    fun msg tag value => PB_Descriptor_update' msg tag value
   end.
-
-Lemma N_shiftr_lor_shiftl
-  : forall a b n, N.lt (N.log2 b) n ->
-             a = N.shiftr (N.lor (N.shiftl a n) b) n.
-Proof.
-  intros. rewrite N.shiftr_lor.
-  rewrite N.shiftr_shiftl_r by apply N.le_refl.
-  rewrite (N.shiftr_eq_0 b); auto.
-  rewrite N.sub_diag.
-  symmetry.
-  apply N.lor_0_r.
-Qed.
-
-Lemma N_land_lor_shiftl
-  : forall a b n, N.lt (N.log2 b) n ->
-             b = N.land (N.lor (N.shiftl a n) b) (N.ones n).
-Proof.
-  intros.
-  rewrite N.land_lor_distr_l.
-  rewrite N.land_ones.
-  rewrite N.shiftl_mul_pow2.
-  rewrite N.mod_mul by (apply N.pow_nonzero; easy).
-  rewrite N.land_ones_low by auto.
-  apply N.lor_0_l.
-Qed.
-
-Lemma decides_N_eq
-  : forall (n n' : N),
-    decides (N.eqb n n') (n = n').
-Proof.
-  unfold decides, If_Then_Else; intros;
-    destruct (N.eqb_spec n n'); auto.
-Qed.
-Hint Resolve decides_N_eq : decide_data_invariant_db.
 
 Inductive PB_IRElm : Type :=
 | Build_PB_IRElm : N ->
@@ -867,6 +817,7 @@ Inductive PB_IRElm : Type :=
                      list PB_IRElm ->
                      PB_IRElm.
 
+(* Induction principle for IR Element. *)
 Section PB_IRElm_induction.
   Variable P : PB_IRElm -> Prop.
   Hypothesis f1 : forall n w s, P (Build_PB_IRElm n w (inl s)).
@@ -881,6 +832,7 @@ Section PB_IRElm_induction.
   Defined.
 End PB_IRElm_induction.
 
+(* Helper functions for accessing element's fields. *)
 Definition PB_IRTag (elm : PB_IRElm) :=
   let (t, _, _) := elm in t.
 
@@ -893,21 +845,22 @@ Definition PB_IRVal (elm : PB_IRElm) :=
               list (PB_WireType_denote (PB_IRType elm)) +
               list PB_IRElm) := elm in v.
 
-Fixpoint PB_IRElm_OK (desc : PB_Message) (elm : PB_IRElm) :=
+(* Well-formedness of IR Element. *)
+Fixpoint PB_IRElm_OK (desc : PB_Descriptor) (elm : PB_IRElm) :=
   match elm with
   | Build_PB_IRElm t ty val =>
-    match PB_Message_boundedTag desc t with
+    match PB_Descriptor_boundedTag desc t with
     | inl tag =>
-      match PB_Message_tagToType tag with
-      | PB_Singular (PB_Primitive pty) =>
+      match PB_Descriptor_tagToType tag with
+      | PB_Singular (PB_Base pty) =>
         match val with
-        | inl (inl _) => PB_PrimitiveType_toWireType pty = ty
+        | inl (inl _) => PB_BaseType_toWireType pty = ty
         | _ => False
         end
-      | PB_Repeated (PB_Primitive pty) =>
+      | PB_Repeated (PB_Base pty) =>
         match val with
-        | inl (inl _) => PB_PrimitiveType_toWireType pty = ty
-        | inl (inr _) => PB_PrimitiveType_toWireType pty = ty /\ ty <> PB_LengthDelimited
+        | inl (inl _) => PB_BaseType_toWireType pty = ty
+        | inl (inr _) => PB_BaseType_toWireType pty = ty /\ ty <> PB_LengthDelimited
         | _ => False
         end
       | PB_Singular (PB_Embedded desc')
@@ -931,7 +884,8 @@ Fixpoint PB_IRElm_OK (desc : PB_Message) (elm : PB_IRElm) :=
     end
   end.
 
-Lemma PB_IRElm_OK_equiv (desc : PB_Message) (ir : list PB_IRElm)
+(* Work around for a weired problem. *)
+Lemma PB_IRElm_OK_equiv (desc : PB_Descriptor) (ir : list PB_IRElm)
   : (fix IR_OK ir :=
        match ir with
        | nil => True
@@ -949,7 +903,7 @@ Proof.
   }
 Qed.
 
-
+(* Just a helper function to get the right wire type for encoding. *)
 Definition PB_IRElm_toWireType (elm : PB_IRElm) :=
   match PB_IRVal elm with
   | inl (inl _) => PB_IRType elm
@@ -958,285 +912,34 @@ Definition PB_IRElm_toWireType (elm : PB_IRElm) :=
 
 Local Opaque PB_LengthDelimited_decode.
 Local Opaque Varint_decode.
-Section PB_IRElm_body.
 
-  Variable format : funType [PB_IRElm; CacheFormat] (ByteString * CacheFormat).
-  Variable decode : PB_Message -> DecodeM PB_IRElm ByteString.
-  Variable format_some : forall d b ce ce', format d ce ↝ (b, ce') -> lt 0 (bin_measure b).
-  Variable format_sz_eq : forall x b1 b2 ce1 ce1' ce2 ce2', format x ce1 ↝ (b1, ce1') ->
-                                                       format x ce2 ↝ (b2, ce2') ->
-                                                       bin_measure b1 = bin_measure b2.
-  Variable format_byte : forall d b ce ce', format d ce ↝ (b, ce') -> bin_measure b mod 8 = 0.
-  Variable P : CacheDecode -> Prop.
-  Variable P_OK : cache_inv_Property P (fun P => forall b cd, P cd -> P (addD cd b)).
-  Variable n : nat.
-  Variable decode_correct : forall b,
-      lt (bin_measure b) n ->
-      forall desc', CorrectDecoder' _ (PB_IRElm_OK desc') (fun _ _ => True) format (decode desc') P b.
+(* Format the value of an element. *)
+Definition PB_IRVal_format
+           (format : funType [PB_IRElm; CacheFormat] (ByteString * CacheFormat))
+  : FormatM PB_IRElm ByteString :=
+  fun elm =>
+    match elm with
+    | Build_PB_IRElm _ ty val =>
+      match val with
+      | inl (inl v) => PB_WireType_format ty v
+      | inl (inr l) => PB_LengthDelimited_format (PB_WireType_format ty) l
+      | inr ir => PB_LengthDelimited_format format (rev ir)
+      end
+    end.
 
-  Definition PB_IRVal_format 
-    : FormatM PB_IRElm ByteString :=
-    fun elm =>
-      match elm with
-      | Build_PB_IRElm _ ty val =>
-        match val with
-        | inl (inl v) => PB_WireType_format ty v
-        | inl (inr l) => PB_LengthDelimited_format (PB_WireType_format ty) l
-        | inr ir => PB_LengthDelimited_format format (rev ir)
-        end
-      end.
+Definition PB_IRElm_format_body
+           (format : funType [PB_IRElm; CacheFormat] (ByteString * CacheFormat))
+           (elm : PB_IRElm) :=
+  Varint_format (N.lor
+                   (N.shiftl (PB_IRTag elm) 3)
+                   (PB_WireType_val (PB_IRElm_toWireType elm)))
+  ThenC PB_IRVal_format format elm
+  DoneC.
 
-  (* :TODO: can we synthesize this? *)
-  Definition PB_IRVal_decode
-             (desc : PB_Message)
-             (t : N) (w : N)
-    : DecodeM PB_IRElm ByteString :=
-    fun b cd =>
-      match PB_WireType_val_inv w with
-      | inleft wty =>
-        match PB_Message_boundedTag desc t with
-        | inl tag =>
-          match PB_Message_tagToType tag with
-          | PB_Singular (PB_Primitive pty) =>
-            if PB_WireType_eq_dec (PB_PrimitiveType_toWireType pty) wty then
-              `(v, b', cd') <- PB_WireType_decode wty b cd;
-                Some (Build_PB_IRElm t wty (inl (inl v)), b', cd')
-            else None
-          | PB_Repeated (PB_Primitive pty) =>
-            if PB_WireType_eq_dec (PB_PrimitiveType_toWireType pty) wty then
-              `(v, b', cd') <- PB_WireType_decode wty b cd;
-                Some (Build_PB_IRElm t wty (inl (inl v)), b', cd')
-            else if PB_WireType_eq_dec PB_LengthDelimited wty then
-                   let wty := (PB_PrimitiveType_toWireType pty) in
-                   `(l, b', cd') <- PB_LengthDelimited_decode (PB_WireType_decode wty) b cd;
-                     Some (Build_PB_IRElm t wty (inl (inr l)), b', cd')
-                 else None
-          | PB_Singular (PB_Embedded desc')
-          | PB_Repeated (PB_Embedded desc') =>
-            if PB_WireType_eq_dec PB_LengthDelimited wty then
-              `(ir, b', cd') <- PB_LengthDelimited_decode (decode desc') b cd;
-                Some (Build_PB_IRElm t PB_LengthDelimited (inr (rev ir)), b', cd')
-            else None
-          end
-        | inr tag =>
-          if PB_FieldTag_OK_dec (uindex tag) then
-            `(v, b', cd') <- PB_WireType_decode wty b cd;
-              Some (Build_PB_IRElm t wty (inl (inl v)), b', cd')
-          else None
-        end
-      | inright _ => None
-      end.
-
-  Local Opaque PB_LengthDelimited_decode.
-  Local Opaque Varint_decode.
-  Theorem PB_IRVal_decode_correct
-          (desc : PB_Message)
-    : forall (t : N) (w : N) b,
-      lt (bin_measure b) (S n) ->
-      CorrectDecoder' _
-                     (fun elm => PB_IRTag elm = t /\
-                              PB_WireType_val (PB_IRElm_toWireType elm) = w /\
-                              PB_IRElm_OK desc elm)
-                     (fun _ _ => True)
-                     PB_IRVal_format (PB_IRVal_decode desc t w) P b.
-  Proof.
-    unfold PB_IRElm_OK, PB_IRVal_format, PB_IRVal_decode, PB_IRElm_toWireType. simpl.
-    destruct desc as [n' desc].
-    intros ? ? ? pf. split; intros.
-    - intuition. destruct data as [tag wty val].
-      destruct PB_WireType_val_inv eqn:?; subst;
-        rewrite PB_WireType_val_inv_correct in Heqs; [| easy].
-      simpl in *. subst.
-      destruct PB_Message_boundedTag eqn:?. {
-        destruct PB_Message_tagToType eqn:?; destruct p0.
-        - destruct val; [destruct s |]; try easy. injections.
-          destruct PB_WireType_eq_dec; [| easy].
-          edestruct PB_WireType_decode_correct as [[? [? [? ?]]] _]; eauto.
-          rewrite H0. simpl. eauto.
-        - destruct val; [easy |]. injections. intuition.
-          destruct PB_WireType_eq_dec; [| easy]. subst.
-          edestruct (PB_LengthDelimited_decode_correct' (A:=PB_IRElm)) as [[? [? [? ?]]] _]; eauto.
-          intros. eapply decode_correct. auto.
-          instantiate (1 := p0).
-          intro. rewrite <- in_rev.
-          apply PB_IRElm_OK_equiv. apply H3.
-          eapply SizedList_predicate_rest_True.
-          rewrite H0. simpl. rewrite rev_involutive. eauto.
-        - destruct val; try easy. injections.
-          destruct PB_WireType_eq_dec.
-          + destruct s; intuition; subst; [| easy].
-            edestruct PB_WireType_decode_correct as [[? [? [? ?]]] _]; eauto.
-            rewrite H0. simpl. eauto.
-          + destruct s; try easy. destruct PB_WireType_eq_dec; try easy. intuition. subst.
-            edestruct (PB_LengthDelimited_decode_correct (A:=(PB_WireType_denote (PB_PrimitiveType_toWireType p0))))
-              as [[? [? [? ?]]] _];
-              eauto using PB_WireType_format_sz_eq, PB_WireType_format_byte,
-              PB_WireType_format_some, PB_WireType_decode_correct.
-            intuition. eapply SizedList_predicate_rest_True.
-            rewrite H0. simpl. eauto.
-        - destruct val; [easy |]. injections. intuition.
-          destruct PB_WireType_eq_dec; [| easy]. subst.
-          edestruct (PB_LengthDelimited_decode_correct' (A:=PB_IRElm))
-            as [[? [? [? ?]]] _]; eauto. intros. apply decode_correct. auto.
-          instantiate (1 := p0). intro. rewrite <- in_rev. apply PB_IRElm_OK_equiv. apply H3.
-          eapply SizedList_predicate_rest_True.
-          rewrite H0. simpl. rewrite rev_involutive. eauto.
-      } {
-        destruct val; [destruct s |]; try easy. injections.
-        edestruct PB_WireType_decode_correct as [[? [? [? ?]]] _]; eauto.
-        simpl in *. rewrite H0. simpl.
-        destruct PB_FieldTag_OK_dec eqn:?.
-        eauto.
-        apply PB_FieldTag_OK_false_iff in Heqb0.
-        easy.
-      }
-    - destruct data as [tag wty val].
-      destruct PB_WireType_val_inv eqn:?; [| easy].
-      apply PB_WireType_val_inv_correct' in Heqs.
-      simpl in *.
-      destruct PB_Message_boundedTag eqn:?. {
-        destruct PB_Message_tagToType eqn:?; destruct p0.
-        - destruct PB_WireType_eq_dec; [| easy]. decode_opt_to_inv.
-          subst. existT_eq_dec; try apply PB_WireType_eq_dec.
-          subst. simpl.
-          edestruct PB_WireType_decode_correct as [_ [? [? [? [? [? [? ?]]]]]]]; eauto.
-          intuition. eexists _, _. intuition; eauto.
-          rewrite Heqs0.
-          destruct PB_Message_tagToType; destruct p; injections; easy.
-        - destruct PB_WireType_eq_dec; [| easy]. decode_opt_to_inv.
-          subst. existT_eq_dec; try apply PB_WireType_eq_dec.
-          subst. simpl.
-          edestruct (PB_LengthDelimited_decode_correct' (A:=PB_IRElm)) as [_ [? [? [? [? [? [? ?]]]]]]]; eauto.
-          intros. apply decode_correct. auto.
-          intuition. eexists _, _. intuition; eauto. rewrite rev_involutive. eauto. rewrite Heqs0.
-          destruct PB_Message_tagToType; destruct p; injections; try easy.
-          intuition. apply (PB_IRElm_OK_equiv p0). intro. rewrite <- in_rev. eauto.
-        - destruct PB_WireType_eq_dec. decode_opt_to_inv.
-          subst. existT_eq_dec; try apply PB_WireType_eq_dec.
-          subst. simpl.
-          edestruct PB_WireType_decode_correct as [_ [? [? [? [? [? [? ?]]]]]]]; eauto.
-          intuition. eexists _, _. intuition; eauto. rewrite Heqs0.
-          destruct PB_Message_tagToType; destruct p; injections; easy.
-          destruct PB_WireType_eq_dec; [| easy]. decode_opt_to_inv.
-          subst. existT_eq_dec; try apply PB_WireType_eq_dec.
-          subst. simpl.
-          edestruct (PB_LengthDelimited_decode_correct (A:=(PB_WireType_denote (PB_PrimitiveType_toWireType p0))))
-            as [_ [? [? [? [? [? [? ?]]]]]]];
-            eauto using PB_WireType_format_sz_eq, PB_WireType_format_byte,
-            PB_WireType_format_some, PB_WireType_decode_correct.
-          intuition. eexists _, _. intuition; eauto. rewrite Heqs0.
-          destruct PB_Message_tagToType; destruct p; injections; easy.
-        - destruct PB_WireType_eq_dec; [| easy]. decode_opt_to_inv.
-          subst. existT_eq_dec; try apply PB_WireType_eq_dec.
-          subst. simpl.
-          edestruct (PB_LengthDelimited_decode_correct' (A:=PB_IRElm)) as [_ [? [? [? [? [? [? ?]]]]]]]; eauto.
-          intros. apply decode_correct. auto.
-          intuition. eexists _, _. intuition; eauto. rewrite rev_involutive; eauto. rewrite Heqs0.
-          destruct PB_Message_tagToType; destruct p; injections; try easy.
-          intuition. apply (PB_IRElm_OK_equiv p0). intro. rewrite <- in_rev. eauto.
-      } {
-        destruct PB_FieldTag_OK_dec eqn:?.
-        decode_opt_to_inv.
-        subst.
-        existT_eq_dec; try apply PB_WireType_eq_dec.
-        subst. simpl.
-        edestruct PB_WireType_decode_correct as [_ [? [? [? [? [? [? ?]]]]]]]; eauto.
-        intuition. eexists _, _. intuition; eauto. rewrite Heqs0.
-        apply PB_FieldTag_OK_true_iff in Heqb0. auto.
-        easy.
-      }
-  Qed.
-
-  Definition PB_IRElm_format_body (elm : PB_IRElm) :=
-    Varint_format (N.lor
-                     (N.shiftl (PB_IRTag elm) 3)
-                     (PB_WireType_val (PB_IRElm_toWireType elm)))
-    ThenC PB_IRVal_format elm
-    DoneC.
-
-  (* :TODO: automate this! *)
-  Definition PB_IRElm_decode_body (desc : PB_Message) :=
-    fun (b0 : ByteString) (cd : CacheDecode) =>
-      `(a, b1, d) <- Varint_decode b0 cd;
-        `(a0, b2, d0) <- PB_IRVal_decode desc (N.shiftr a 3) (N.land a 7) b1 d;
-        (if (N.lor (N.shiftl (PB_IRTag a0) 3) (PB_WireType_val (PB_IRElm_toWireType a0)) =? a)%N
-         then Some (a0, b2, d0)
-         else None).
-
-  Definition PB_IRElm_decode_body_correct (desc : PB_Message)
-    : forall b,
-      lt (bin_measure b) (S n) ->
-      CorrectDecoder' _ (PB_IRElm_OK desc) (fun _ _ => True) PB_IRElm_format_body (PB_IRElm_decode_body desc) P b.
-  Proof.
-    unfold PB_IRElm_format_body, PB_IRElm_decode_body.
-    split; intros. {
-      computes_to_inv2.
-      pose proof H3.
-      eapply Varint_decode_correct in H3; eauto. destruct_many.
-      rewrite <- (@mappend_assoc _ ByteStringQueueMonoid). rewrite H3.
-      simpl. eapply PB_IRVal_decode_correct in H3'; eauto. destruct_many.
-      match goal with
-      | H : PB_IRVal_decode _ ?t' ?w' _ _ = _ |- context [PB_IRVal_decode _ ?t ?w] =>
-        replace t with t'; [replace w with w' | ]
-      end.
-      rewrite H7. simpl. rewrite N.eqb_refl. eauto.
-      apply N_land_lor_shiftl. apply PB_WireType_val_3bits.
-      apply N_shiftr_lor_shiftl. apply PB_WireType_val_3bits.
-      apply Varint_format_some in H4.
-      rewrite !(@mappend_measure _ ByteStringQueueMonoid) in H. omega.
-    } {
-      decode_opt_to_inv.
-      match goal with
-      | H : context [if (?a =? ?b)%N then _ else _] |- _ =>
-        destruct (N.eqb_spec a b)
-      end. 2 : easy.
-      injections.
-      eapply Varint_decode_correct in H2; eauto. destruct_many.
-      eapply PB_IRVal_decode_correct in H3; eauto. destruct_many.
-      intuition. eexists _, _. intuition eauto.
-      repeat computes_to_econstructor; eauto.
-      simpl. subst. rewrite <- (@mappend_assoc _ ByteStringQueueMonoid).
-      rewrite (@mempty_right _ ByteStringQueueMonoid). reflexivity.
-      subst. apply Varint_format_some in H4. rewrite mappend_measure in H. omega.
-    }
-  Qed.
-
-  (* Definition PB_IRElm_body_decoder (desc : PB_Message) *)
-  (*   : CorrectDecoderFor (PB_IRElm_OK desc) PB_IRElm_format_body. *)
-  (* Proof. *)
-  (*   unfold PB_IRElm_OK, PB_IRElm_format_body. *)
-  (*   eapply Start_CorrectDecoderFor; simpl. *)
-  (*   - decode_step idtac. *)
-  (*     apply Varint_decode_correct. *)
-  (*     decode_step idtac. *)
-  (*     decode_step idtac. *)
-  (*     decode_step idtac. *)
-  (*     intros. eapply (PB_IRVal_decode_correct desc) *)
-  (*               with (t := N.shiftr proj 3) *)
-  (*                    (w := N.land proj 7). *)
-  (*     intros ? [? ?]. repeat split; eauto; subst. *)
-  (*     apply N_shiftr_lor_shiftl. apply PB_WireType_val_3bits. *)
-  (*     apply N_land_lor_shiftl. apply PB_WireType_val_3bits. *)
-  (*     decode_step idtac. *)
-  (*     decode_step idtac. *)
-  (*   - cbv beta; synthesize_cache_invariant. *)
-  (*   - cbv beta; optimize_decoder_impl. *)
-  (* Defined. *)
-
-  (* Definition PB_IRElm_decode_body (desc : PB_Message) := *)
-  (*   Eval simpl in fst (proj1_sig (PB_IRElm_body_decoder desc)). *)
-
-  (* Definition PB_IRElm_decode_body_correct (desc : PB_Message) *)
-  (*   : CorrectDecoder' _ *)
-  (*                    (PB_IRElm_OK desc) *)
-  (*                    (fun _ _ => True) *)
-  (*                    PB_IRElm_format_body (PB_IRElm_decode_body desc) P b. *)
-  (* Proof. *)
-  (*   destruct (proj2_sig (PB_IRElm_body_decoder desc)) as [? [? ?]]. *)
-  (*   apply H. simpl in *. auto. *)
-  (* Qed. *)
-
-End PB_IRElm_body.
+(* Format a single element. *)
+Definition PB_IRElm_format
+  : FormatM PB_IRElm ByteString :=
+    LeastFixedPoint PB_IRElm_format_body.
 
 Lemma PB_IRElm_format_body_monotone:
   monotonic_function PB_IRElm_format_body.
@@ -1266,14 +969,7 @@ Proof.
   auto. reflexivity.
 Qed.
 
-Definition PB_IRElm_format
-  : FormatM PB_IRElm ByteString :=
-    LeastFixedPoint PB_IRElm_format_body.
-
-Definition PB_IRElm_decode (desc : PB_Message)
-  : DecodeM PB_IRElm ByteString :=
-  FueledFixP PB_IRElm_decode_body desc.
-
+(* IR element can not formatted to empty string. *)
 Theorem PB_IRElm_format_some
   : forall d b ce ce', PB_IRElm_format d ce ↝ (b, ce') -> lt 0 (bin_measure b).
 Proof.
@@ -1285,6 +981,7 @@ Proof.
   rewrite !(@mappend_measure). omega.
 Qed.
 
+(* IR elements are always formatted into the same size. *)
 Theorem PB_IRElm_format_sz_eq
   : forall x b1 b2 ce1 ce1' ce2 ce2',
     PB_IRElm_format x ce1 ↝ (b1, ce1') ->
@@ -1316,6 +1013,7 @@ Proof.
   }
 Qed.
 
+(* IR Elements' binary strings are byte-aligned. *)
 Theorem PB_IRElm_format_byte
   : forall d b ce ce', PB_IRElm_format d ce ↝ (b, ce') -> bin_measure b mod 8 = 0.
 Proof.
@@ -1353,86 +1051,10 @@ Proof.
   }
 Qed.
 
-(* :TODO: generalize this and put it to SizedList module. *)
-Lemma SizedList_decode_continous_pres
-      {A B C} {monoid : Monoid B}
-      (decode_body : (C -> B -> CacheDecode -> option (A * B * CacheDecode)) ->
-                     C -> B -> CacheDecode -> option (A * B * CacheDecode))
-  : forall decode : C -> B -> CacheDecode -> option (A * B * CacheDecode),
-    (forall c b cd a b' cd',
-        decode c b cd = Some (a, b', cd') -> decode_body decode c b cd = Some (a, b', cd')) ->
-    forall sz c b cd a b' cd',
-      SizedList_decode (decode c) sz b cd = Some (a, b', cd') ->
-      SizedList_decode (decode_body decode c) sz b cd = Some (a, b', cd').
-Proof.
-  unfold SizedList_decode, SizedList_decode_body, FueledFixP in *.
-  intros ? ? ? ? ?. revert sz c. generalize (bin_measure b). intro. revert b.
-  induction n; simpl; intros. destruct sz; auto. decode_opt_to_inv.
-  apply H in H0. rewrite H0. simpl. auto.
-  destruct sz. auto.
-  decode_opt_to_inv. apply H in H0. rewrite H0. simpl.
-  destruct lt_dec. auto.
-  decode_opt_to_inv. apply IHn in H1. subst. simpl in *. rewrite H1.
-  simpl. auto.
-Qed.
-
-Local Transparent PB_LengthDelimited_decode.
-Lemma PB_LengthDelimited_decode_continous_pres
-      {A B C} {monoid : Monoid B} {monoidUnit : QueueMonoidOpt monoid bool}
-      (decode_body : (C -> B -> CacheDecode -> option (A * B * CacheDecode)) ->
-                     C -> B -> CacheDecode -> option (A * B * CacheDecode))
-  : forall decode : C -> B -> CacheDecode -> option (A * B * CacheDecode),
-    (forall c b cd a b' cd',
-        decode c b cd = Some (a, b', cd') -> decode_body decode c b cd = Some (a, b', cd')) ->
-    forall c b cd a b' cd',
-      PB_LengthDelimited_decode (decode c) b cd = Some (a, b', cd') ->
-      PB_LengthDelimited_decode (decode_body decode c) b cd = Some (a, b', cd').
-Proof.
-  unfold PB_LengthDelimited_decode. intros.
-  decode_opt_to_inv. rewrite H0. simpl. subst.
-  apply SizedList_decode_continous_pres; eauto.
-Qed.
-
-Local Opaque PB_LengthDelimited_decode.
-Definition PB_IRElm_decode_correct (desc : PB_Message)
-           {P : CacheDecode -> Prop}
-           (P_OK : cache_inv_Property P (fun P => forall b cd, P cd -> P (addD cd b)))
-  : CorrectDecoder _
-                   (PB_IRElm_OK desc)
-                   (fun _ _ => True)
-                   PB_IRElm_format (PB_IRElm_decode desc) P.
-Proof.
-  unfold PB_IRElm_format, PB_IRElm_decode.
-  eapply fix_format_correctP; eauto. apply PB_IRElm_format_body_monotone.
-  intros _. intros.
-  eapply PB_IRElm_decode_body_correct;
-    eauto using PB_IRElm_format_some, PB_IRElm_format_byte, PB_IRElm_format_sz_eq.
-
-  intros.
-  unfold PB_IRElm_decode_body at 1.
-  decode_opt_to_inv. rewrite H0. simpl.
-  unfold PB_IRVal_decode.
-  unfold PB_IRVal_decode in *.
-  destruct PB_WireType_val_inv; [| easy].
-  destruct PB_Message_boundedTag. {
-    destruct PB_Message_tagToType; destruct p0.
-    - rewrite H1. simpl. auto.
-    - destruct PB_WireType_eq_dec; [| easy].
-      decode_opt_to_inv. eapply PB_LengthDelimited_decode_continous_pres in H1; eauto.
-      rewrite H1. simpl. subst. auto.
-    - rewrite H1. auto.
-    - destruct PB_WireType_eq_dec; [| easy].
-      decode_opt_to_inv. eapply PB_LengthDelimited_decode_continous_pres in H1; eauto.
-      rewrite H1. simpl. subst. auto.
-  } {
-    rewrite H1. simpl. auto.
-  }
-Qed.
-Local Transparent Varint_decode.
-Local Transparent PB_LengthDelimited_decode.
-
 Definition PB_IR := list PB_IRElm.
 
+(* The measurement of IR is not the length of the list but includes the length
+   of the sub-IR. *)
 Definition PB_IR_measure' f :=
   fix ir_measure (ir : PB_IR) :=
     match ir with
@@ -1462,6 +1084,7 @@ Proof.
   omega.
 Qed.
 
+(* IR is a monoid. *)
 Instance PB_IR_monoid : Monoid PB_IR :=
   {| mappend := @app _;
      bin_measure := PB_IR_measure;
@@ -1486,155 +1109,157 @@ Proof.
   omega.
 Qed.
 
-Inductive PB_IR_refine
-  : forall {desc : PB_Message}, PB_Message_denote desc -> PB_IR -> PB_Message_denote desc -> Prop :=
+(* The key inference rules for the relation msg' |- ir ~= msg *)
+Inductive PB_IR_transit
+  : forall {desc : PB_Descriptor}, PB_Descriptor_denote desc -> PB_IR -> PB_Descriptor_denote desc -> Prop :=
 | PB_IR_nil desc :
-    forall msg : PB_Message_denote desc, PB_IR_refine msg nil msg
+    forall msg : PB_Descriptor_denote desc, PB_IR_transit msg nil msg
 | PB_IR_singular desc :
-    forall (msg' : PB_Message_denote desc) ir (msg : PB_Message_denote desc),
-      PB_IR_refine msg' ir msg ->
-      forall (t : BoundedTag desc) (pty : PB_PrimitiveType)
-        (pf : PB_Message_tagToType t = PB_Singular (PB_Primitive pty))
-        (v : PB_Type_denote (PB_Singular (PB_Primitive pty))),
-        PB_IR_refine msg'
+    forall (msg' : PB_Descriptor_denote desc) ir (msg : PB_Descriptor_denote desc),
+      PB_IR_transit msg' ir msg ->
+      forall (t : BoundedTag desc) (pty : PB_BaseType)
+        (pf : PB_Descriptor_tagToType t = PB_Singular (PB_Base pty))
+        (v : PB_Type_denote (PB_Singular (PB_Base pty))),
+        PB_IR_transit msg'
                      ((Build_PB_IRElm (bindex t)
-                                      (PB_PrimitiveType_toWireType pty)
+                                      (PB_BaseType_toWireType pty)
                                       (inl (inl v))) :: ir)
-                     (PB_Message_update msg t (eq_rect_r _ v pf))
+                     (PB_Descriptor_update msg t (eq_rect_r _ v pf))
 | PB_IR_repeated_cons desc :
-    forall (msg' : PB_Message_denote desc) ir (msg : PB_Message_denote desc),
-      PB_IR_refine msg' ir msg ->
-      forall (t : BoundedTag desc) (pty : PB_PrimitiveType)
-        (pf : PB_Message_tagToType t = PB_Repeated (PB_Primitive pty))
-        (v : PB_Type_denote (PB_Singular (PB_Primitive pty))),
-        PB_IR_refine msg'
+    forall (msg' : PB_Descriptor_denote desc) ir (msg : PB_Descriptor_denote desc),
+      PB_IR_transit msg' ir msg ->
+      forall (t : BoundedTag desc) (pty : PB_BaseType)
+        (pf : PB_Descriptor_tagToType t = PB_Repeated (PB_Base pty))
+        (v : PB_Type_denote (PB_Singular (PB_Base pty))),
+        PB_IR_transit msg'
                      ((Build_PB_IRElm (bindex t)
-                                      (PB_PrimitiveType_toWireType pty)
+                                      (PB_BaseType_toWireType pty)
                                       (inl (inl v))) :: ir)
-                     (PB_Message_update msg t
+                     (PB_Descriptor_update msg t
                                         (eq_rect_r
                                            _
-                                           ((eq_rect _ _ (PB_Message_lookup msg t) _ pf) ++ [v])
+                                           ((eq_rect _ _ (PB_Descriptor_lookup msg t) _ pf) ++ [v])
                                            pf))
 | PB_IR_repeated_app desc :
-    forall (msg' : PB_Message_denote desc) ir (msg : PB_Message_denote desc),
-      PB_IR_refine msg' ir msg ->
-      forall (t : BoundedTag desc) (pty : PB_PrimitiveType)
-        (pf : PB_Message_tagToType t = PB_Repeated (PB_Primitive pty))
-        (v : PB_Type_denote (PB_Repeated (PB_Primitive pty))),
-        PB_PrimitiveType_toWireType pty <> PB_LengthDelimited ->
-        PB_IR_refine msg'
+    forall (msg' : PB_Descriptor_denote desc) ir (msg : PB_Descriptor_denote desc),
+      PB_IR_transit msg' ir msg ->
+      forall (t : BoundedTag desc) (pty : PB_BaseType)
+        (pf : PB_Descriptor_tagToType t = PB_Repeated (PB_Base pty))
+        (v : PB_Type_denote (PB_Repeated (PB_Base pty))),
+        PB_BaseType_toWireType pty <> PB_LengthDelimited ->
+        PB_IR_transit msg'
                      ((Build_PB_IRElm (bindex t)
-                                      (PB_PrimitiveType_toWireType pty)
+                                      (PB_BaseType_toWireType pty)
                                       (inl (inr v))) :: ir)
-                     (PB_Message_update msg t
+                     (PB_Descriptor_update msg t
                                         (eq_rect_r
                                            _
-                                           ((eq_rect _ _ (PB_Message_lookup msg t) _ pf) ++ v)
+                                           ((eq_rect _ _ (PB_Descriptor_lookup msg t) _ pf) ++ v)
                                            pf))
 | PB_IR_unknown desc :
-    forall (msg' : PB_Message_denote desc) ir (msg : PB_Message_denote desc),
-      PB_IR_refine msg' ir msg ->
+    forall (msg' : PB_Descriptor_denote desc) ir (msg : PB_Descriptor_denote desc),
+      PB_IR_transit msg' ir msg ->
       forall (t : UnboundedTag desc) (wty : PB_WireType)
         (v : PB_WireType_denote wty),
         PB_FieldTag_OK (uindex t) ->
-        PB_IR_refine msg'
+        PB_IR_transit msg'
                      ((Build_PB_IRElm (uindex t)
                                       wty
                                       (inl (inl v))) :: ir)
                      msg
 | PB_IR_embedded_none desc :
-    forall (msg' : PB_Message_denote desc) ir (msg : PB_Message_denote desc),
-      PB_IR_refine msg' ir msg ->
-      forall (t : BoundedTag desc) (desc' : PB_Message)
-        (pf : PB_Message_tagToType t = PB_Singular (PB_Embedded desc'))
-        v (msg'' : PB_Message_denote desc'),
-        eq_rect _ _ (PB_Message_lookup msg t) _ pf = None ->
-        PB_IR_refine (PB_Message_default desc') v msg'' ->
-        PB_IR_refine msg'
+    forall (msg' : PB_Descriptor_denote desc) ir (msg : PB_Descriptor_denote desc),
+      PB_IR_transit msg' ir msg ->
+      forall (t : BoundedTag desc) (desc' : PB_Descriptor)
+        (pf : PB_Descriptor_tagToType t = PB_Singular (PB_Embedded desc'))
+        v (msg'' : PB_Descriptor_denote desc'),
+        eq_rect _ _ (PB_Descriptor_lookup msg t) _ pf = None ->
+        PB_IR_transit (PB_Descriptor_default desc') v msg'' ->
+        PB_IR_transit msg'
                      ((Build_PB_IRElm (bindex t)
                                       PB_LengthDelimited
                                       (inr v)) :: ir)
-                     (PB_Message_update msg t
+                     (PB_Descriptor_update msg t
                                         (eq_rect_r _ (Some msg'') pf))
 | PB_IR_embedded_some desc :
-    forall (msg' : PB_Message_denote desc) ir (msg : PB_Message_denote desc),
-      PB_IR_refine msg' ir msg ->
-      forall (t : BoundedTag desc) (desc' : PB_Message)
-        (pf : PB_Message_tagToType t = PB_Singular (PB_Embedded desc'))
-        v (msg'' msg''' : PB_Message_denote desc'),
-        eq_rect _ _ (PB_Message_lookup msg t) _ pf = Some msg'' ->
-        PB_IR_refine msg'' v msg''' ->
-        PB_IR_refine msg'
+    forall (msg' : PB_Descriptor_denote desc) ir (msg : PB_Descriptor_denote desc),
+      PB_IR_transit msg' ir msg ->
+      forall (t : BoundedTag desc) (desc' : PB_Descriptor)
+        (pf : PB_Descriptor_tagToType t = PB_Singular (PB_Embedded desc'))
+        v (msg'' msg''' : PB_Descriptor_denote desc'),
+        eq_rect _ _ (PB_Descriptor_lookup msg t) _ pf = Some msg'' ->
+        PB_IR_transit msg'' v msg''' ->
+        PB_IR_transit msg'
                      ((Build_PB_IRElm (bindex t)
                                       PB_LengthDelimited
                                       (inr v)) :: ir)
-                     (PB_Message_update msg t
+                     (PB_Descriptor_update msg t
                                         (eq_rect_r _ (Some msg''') pf))
 | PB_IR_repeated_embedded desc :
-    forall (msg' : PB_Message_denote desc) ir (msg : PB_Message_denote desc),
-      PB_IR_refine msg' ir msg ->
-      forall (t : BoundedTag desc) (desc' : PB_Message)
-        (pf : PB_Message_tagToType t = PB_Repeated (PB_Embedded desc'))
-        v (msg'' : PB_Message_denote desc'),
-        PB_IR_refine (PB_Message_default desc') v msg'' ->
-        PB_IR_refine msg'
+    forall (msg' : PB_Descriptor_denote desc) ir (msg : PB_Descriptor_denote desc),
+      PB_IR_transit msg' ir msg ->
+      forall (t : BoundedTag desc) (desc' : PB_Descriptor)
+        (pf : PB_Descriptor_tagToType t = PB_Repeated (PB_Embedded desc'))
+        v (msg'' : PB_Descriptor_denote desc'),
+        PB_IR_transit (PB_Descriptor_default desc') v msg'' ->
+        PB_IR_transit msg'
                      ((Build_PB_IRElm (bindex t)
                                       PB_LengthDelimited
                                       (inr v)) :: ir)
-                     (PB_Message_update msg t
+                     (PB_Descriptor_update msg t
                                         (eq_rect_r
                                            _
-                                           ((eq_rect _ _ (PB_Message_lookup msg t) _ pf) ++ [msg''])
+                                           ((eq_rect _ _ (PB_Descriptor_lookup msg t) _ pf) ++ [msg''])
                                            pf))
 .
 
-Ltac PB_IR_refine_inv_step :=
+Ltac PB_IR_transit_inv_step :=
   match goal with
   | H : bindex ?a = bindex _ |- _ => apply BoundedTag_inj in H; [subst a | solve [eauto]]
   | H : uindex _ = bindex _ |- _ => symmetry in H
   | H : bindex _ = uindex _ |- _ => apply BoundedTag_not_unbounded in H; inversion H
-  | H : PB_Message_tagToType ?t = ?c1 (?c2 ?a),
-        H' : PB_Message_tagToType ?t = ?c1 (?c2 ?b) |- _ => progress replace b with a in * by congruence
+  | H : PB_Descriptor_tagToType ?t = ?c1 (?c2 ?a),
+        H' : PB_Descriptor_tagToType ?t = ?c1 (?c2 ?b) |- _ => progress replace b with a in * by congruence
   | H : existT _ _ _ = existT _ _ _ |- _  =>
     apply inj_pair2_eq_dec in H;
-    [| clear H; try apply PB_Message_eq_dec || apply PB_WireType_eq_dec];
+    [| clear H; try apply PB_Descriptor_eq_dec || apply PB_WireType_eq_dec];
     subst
   | H : ?a = Some _, H' : ?b = None |- _ => progress replace a with b in *; [congruence | clear H H']
   | H : ?a = Some _, H' : ?b = Some _ |- _ => progress replace a with b in *; [substss; injections | clear H H']
   | |- ?a = ?b => progress f_equal; eauto; try apply (UIP_dec PB_Type_eq_dec)
-  | _ => eauto using eq_sym, PB_Message_OK_sub_tagToType; easy || congruence
+  | _ => eauto using eq_sym, PB_Descriptor_OK_sub_tagToType; easy || congruence
   end.
 
-Ltac PB_IR_refine_inv hyp :=
-  inversion hyp; repeat PB_IR_refine_inv_step.
+Ltac PB_IR_transit_inv hyp :=
+  inversion hyp; repeat PB_IR_transit_inv_step.
 
-Theorem PB_IR_refine_deterministic
+(* Some properties for the relation. *)
+Theorem PB_IR_transit_deterministic
   : forall desc,
-    PB_Message_OK desc ->
-    forall (msg' msg1 msg2 : PB_Message_denote desc) ir,
-      PB_IR_refine msg' ir msg1 ->
-      PB_IR_refine msg' ir msg2 ->
+    PB_Descriptor_OK desc ->
+    forall (msg' msg1 msg2 : PB_Descriptor_denote desc) ir,
+      PB_IR_transit msg' ir msg1 ->
+      PB_IR_transit msg' ir msg2 ->
       msg1 = msg2.
 Proof.
-  intros. induction H0; PB_IR_refine_inv H1.
+  intros. induction H0; PB_IR_transit_inv H1.
 Qed.
 
-Ltac PB_IR_refine_inv_step_ext :=
+Ltac PB_IR_transit_inv_step_ext :=
   match goal with
-  | |- PB_IR_refine ?a nil ?b => replace a with b; [constructor |]
-  | _ => eauto using eq_sym, PB_Message_OK_sub_tagToType, PB_IR_refine_deterministic
+  | |- PB_IR_transit ?a nil ?b => replace a with b; [constructor |]
+  | _ => eauto using eq_sym, PB_Descriptor_OK_sub_tagToType, PB_IR_transit_deterministic
   end.
 
-Ltac PB_IR_refine_inv hyp ::=
-  inversion hyp; repeat first [PB_IR_refine_inv_step | PB_IR_refine_inv_step_ext].
+Ltac PB_IR_transit_inv hyp ::=
+  inversion hyp; repeat first [PB_IR_transit_inv_step | PB_IR_transit_inv_step_ext].
 
-Theorem PB_IR_refine_trans
+Theorem PB_IR_transit_trans
   : forall desc,
-    PB_Message_OK desc ->
-    forall (msg1 msg2 msg3 : PB_Message_denote desc) (ir1 ir2 ir3 : PB_IR),
-    PB_IR_refine msg1 ir1 msg2 ->
-    (PB_IR_refine msg2 ir2 msg3 <-> PB_IR_refine msg1 (ir2 ++ ir1) msg3).
+    PB_Descriptor_OK desc ->
+    forall (msg1 msg2 msg3 : PB_Descriptor_denote desc) (ir1 ir2 ir3 : PB_IR),
+    PB_IR_transit msg1 ir1 msg2 ->
+    (PB_IR_transit msg2 ir2 msg3 <-> PB_IR_transit msg1 (ir2 ++ ir1) msg3).
 Proof.
   split; intros. {
     induction H1; simpl; eauto; try solve [constructor; eauto].
@@ -1647,7 +1272,7 @@ Proof.
     induction H1; simpl; intros.
     all : destruct ir2; simpl in Heql; injections; subst;
       [match goal with
-       | H : PB_IR_refine _ _ ?a |- PB_IR_refine ?a _ _ => solve [PB_IR_refine_inv H]
+       | H : PB_IR_transit _ _ ?a |- PB_IR_transit ?a _ _ => solve [PB_IR_transit_inv H]
        end |
        match goal with
        | H : _ = Some _ |- _ => eapply PB_IR_embedded_some; eauto
@@ -1656,10 +1281,26 @@ Proof.
   }
 Qed.
 
-Definition PB_Message_IR_format_body
-           (format : funType_dep [PB_Message_denote; PB_Message_denote; fun _ => CacheFormat]
+(* We define the format directly from this relation. This is the stronger
+   version. *)
+Definition PB_Descriptor_IR_format_ref' (desc : PB_Descriptor) msg'
+  : FormatM (PB_Descriptor_denote desc) PB_IR :=
+  fun msg _ => {b | PB_IR_transit msg' (fst b) msg}.
+Arguments PB_Descriptor_IR_format_ref' /.
+
+(* This is the format we want, which is just a special case of the stronger
+   version. *)
+Definition PB_Descriptor_IR_format_ref (desc : PB_Descriptor)
+  : FormatM (PB_Descriptor_denote desc) PB_IR :=
+  PB_Descriptor_IR_format_ref' desc (PB_Descriptor_default desc).
+
+(* Here is an alternative definition of the previous relation. They are
+   equivalent as we show below. This is a byproduct of our another experiment
+   but we end up proving the correctness theorem using this definition. *)
+Definition PB_Descriptor_IR_format_body
+           (format : funType_dep [PB_Descriptor_denote; PB_Descriptor_denote; fun _ => CacheFormat]
                                  (PB_IR * CacheFormat))
-  : funType_dep [PB_Message_denote; PB_Message_denote; fun _ => CacheFormat]
+  : funType_dep [PB_Descriptor_denote; PB_Descriptor_denote; fun _ => CacheFormat]
                 (PB_IR * CacheFormat) :=
   fun desc msg' msg _ b =>
     let (ir, _) := b in
@@ -1667,40 +1308,40 @@ Definition PB_Message_IR_format_body
     (msg' = msg /\ ir = nil) \/
     (* singular *)
     (exists ir1 msg1 t pty
-       (v : PB_Type_denote (PB_Singular (PB_Primitive pty)))
-       (pf : PB_Message_tagToType t = PB_Singular (PB_Primitive pty)) ce1 ce2,
+       (v : PB_Type_denote (PB_Singular (PB_Base pty)))
+       (pf : PB_Descriptor_tagToType t = PB_Singular (PB_Base pty)) ce1 ce2,
         format _ msg' msg1 ce1 (ir1, ce2) /\
         ir = (Build_PB_IRElm (bindex t)
-                             (PB_PrimitiveType_toWireType pty)
+                             (PB_BaseType_toWireType pty)
                              (inl (inl v))) :: ir1 /\
-        msg = PB_Message_update msg1 t
+        msg = PB_Descriptor_update msg1 t
                                 (eq_rect_r _ v pf)) \/
     (* repeated_cons *)
     (exists ir1 msg1 t pty
-       (v : PB_Type_denote (PB_Singular (PB_Primitive pty)))
-       (pf : PB_Message_tagToType t = PB_Repeated (PB_Primitive pty)) ce1 ce2,
+       (v : PB_Type_denote (PB_Singular (PB_Base pty)))
+       (pf : PB_Descriptor_tagToType t = PB_Repeated (PB_Base pty)) ce1 ce2,
         format _ msg' msg1 ce1 (ir1, ce2) /\
         ir = (Build_PB_IRElm (bindex t)
-                             (PB_PrimitiveType_toWireType pty)
+                             (PB_BaseType_toWireType pty)
                              (inl (inl v))) :: ir1 /\
-        msg = PB_Message_update msg1 t
+        msg = PB_Descriptor_update msg1 t
                                 (eq_rect_r
                                    _
-                                   ((eq_rect _ _ (PB_Message_lookup msg1 t) _ pf) ++ [v])
+                                   ((eq_rect _ _ (PB_Descriptor_lookup msg1 t) _ pf) ++ [v])
                                    pf)) \/
     (* repeated_app *)
     (exists ir1 msg1 t pty
-       (v : PB_Type_denote (PB_Repeated (PB_Primitive pty)))
-       (pf : PB_Message_tagToType t = PB_Repeated (PB_Primitive pty)) ce1 ce2,
+       (v : PB_Type_denote (PB_Repeated (PB_Base pty)))
+       (pf : PB_Descriptor_tagToType t = PB_Repeated (PB_Base pty)) ce1 ce2,
         format _ msg' msg1 ce1 (ir1, ce2) /\
-        PB_PrimitiveType_toWireType pty <> PB_LengthDelimited /\
+        PB_BaseType_toWireType pty <> PB_LengthDelimited /\
         ir = (Build_PB_IRElm (bindex t)
-                             (PB_PrimitiveType_toWireType pty)
+                             (PB_BaseType_toWireType pty)
                              (inl (inr v))) :: ir1 /\
-        msg = PB_Message_update msg1 t
+        msg = PB_Descriptor_update msg1 t
                                 (eq_rect_r
                                    _
-                                   ((eq_rect _ _ (PB_Message_lookup msg1 t) _ pf) ++ v)
+                                   ((eq_rect _ _ (PB_Descriptor_lookup msg1 t) _ pf) ++ v)
                                    pf)) \/
     (* unknown *)
     (exists ir1 (t : UnboundedTag desc) wty (v : PB_WireType_denote wty) ce1 ce2,
@@ -1710,50 +1351,50 @@ Definition PB_Message_IR_format_body
                              wty
                              (inl (inl v))) :: ir1) \/
     (* embedded_none *)
-    (exists ir1 msg1 t desc' v (msg2 : PB_Message_denote desc')
-       (pf : PB_Message_tagToType t = PB_Singular (PB_Embedded desc')) ce1 ce2 ce3 ce4,
+    (exists ir1 msg1 t desc' v (msg2 : PB_Descriptor_denote desc')
+       (pf : PB_Descriptor_tagToType t = PB_Singular (PB_Embedded desc')) ce1 ce2 ce3 ce4,
         format _ msg' msg1 ce1 (ir1, ce2) /\
-        eq_rect _ _ (PB_Message_lookup msg1 t) _ pf = None /\
-        format _ (PB_Message_default desc') msg2 ce3 (v, ce4) /\
+        eq_rect _ _ (PB_Descriptor_lookup msg1 t) _ pf = None /\
+        format _ (PB_Descriptor_default desc') msg2 ce3 (v, ce4) /\
         ir = (Build_PB_IRElm (bindex t)
                              PB_LengthDelimited
                              (inr v)) :: ir1 /\
-        msg = PB_Message_update msg1 t
+        msg = PB_Descriptor_update msg1 t
                                 (eq_rect_r _ (Some msg2) pf)) \/
     (* embedded_some *)
-    (exists ir1 msg1 t desc' v (msg2 msg3 : PB_Message_denote desc')
-       (pf : PB_Message_tagToType t = PB_Singular (PB_Embedded desc')) ce1 ce2 ce3 ce4,
+    (exists ir1 msg1 t desc' v (msg2 msg3 : PB_Descriptor_denote desc')
+       (pf : PB_Descriptor_tagToType t = PB_Singular (PB_Embedded desc')) ce1 ce2 ce3 ce4,
         format _ msg' msg1 ce1 (ir1, ce2) /\
-        eq_rect _ _ (PB_Message_lookup msg1 t) _ pf = Some msg2 /\
+        eq_rect _ _ (PB_Descriptor_lookup msg1 t) _ pf = Some msg2 /\
         format _ msg2 msg3 ce3 (v, ce4) /\
         ir = (Build_PB_IRElm (bindex t)
                              PB_LengthDelimited
                              (inr v)) :: ir1 /\
-        msg = PB_Message_update msg1 t
+        msg = PB_Descriptor_update msg1 t
                                 (eq_rect_r _ (Some msg3) pf)) \/
     (* repeated_embedded *)
-    (exists ir1 msg1 t desc' v (msg2 : PB_Message_denote desc')
-       (pf : PB_Message_tagToType t = PB_Repeated (PB_Embedded desc')) ce1 ce2 ce3 ce4,
+    (exists ir1 msg1 t desc' v (msg2 : PB_Descriptor_denote desc')
+       (pf : PB_Descriptor_tagToType t = PB_Repeated (PB_Embedded desc')) ce1 ce2 ce3 ce4,
         format _ msg' msg1 ce1 (ir1, ce2) /\
-        format _ (PB_Message_default desc') msg2 ce3 (v, ce4) /\
+        format _ (PB_Descriptor_default desc') msg2 ce3 (v, ce4) /\
         ir = (Build_PB_IRElm (bindex t)
                              PB_LengthDelimited
                              (inr v)) :: ir1 /\
-        msg = PB_Message_update msg1 t
+        msg = PB_Descriptor_update msg1 t
                                 (eq_rect_r
                                    _
-                                   ((eq_rect _ _ (PB_Message_lookup msg1 t) _ pf) ++ [msg2])
+                                   ((eq_rect _ _ (PB_Descriptor_lookup msg1 t) _ pf) ++ [msg2])
                                    pf))
 .
 
 Local Transparent computes_to.
 Local Transparent Pick.
 
-Lemma PB_Message_IR_format_body_monotone
-  : monotonic_function PB_Message_IR_format_body.
+Lemma PB_Descriptor_IR_format_body_monotone
+  : monotonic_function PB_Descriptor_IR_format_body.
 Proof.
   unfold monotonic_function. simpl. intros.
-  unfold PB_Message_IR_format_body.
+  unfold PB_Descriptor_IR_format_body.
   intros [ir desc msg' msg ce]. intros [? ?]. unfold computes_to. intros.
   destruct_many;
     let solv n := solve [choose_br n; repeat eexists; eauto; apply H; eauto] in
@@ -1764,36 +1405,29 @@ Proof.
     trial 7.
 Qed.
 
-Definition PB_Message_IR_format_ref' (desc : PB_Message) msg'
-  : FormatM (PB_Message_denote desc) PB_IR :=
-  fun msg _ => {b | PB_IR_refine msg' (fst b) msg}.
-Arguments PB_Message_IR_format_ref' /.
+(* We define the format as a least fixed point. *)
+Definition PB_Descriptor_IR_format' := LeastFixedPoint_dep PB_Descriptor_IR_format_body.
 
-Definition PB_Message_IR_format_ref (desc : PB_Message)
-  : FormatM (PB_Message_denote desc) PB_IR :=
-  PB_Message_IR_format_ref' desc (PB_Message_default desc).
-
-Definition PB_Message_IR_format' := LeastFixedPoint_dep PB_Message_IR_format_body.
-
-Definition PB_Message_IR_format (desc : PB_Message)
-  : FormatM (PB_Message_denote desc) PB_IR :=
+Definition PB_Descriptor_IR_format (desc : PB_Descriptor)
+  : FormatM (PB_Descriptor_denote desc) PB_IR :=
   fun msg =>
-    PB_Message_IR_format' _ (PB_Message_default desc) msg.
+    PB_Descriptor_IR_format' _ (PB_Descriptor_default desc) msg.
 
-Theorem PB_Message_IR_format_eq' (desc : PB_Message)
+(* These two definitions of format are indeed equivalent. *)
+Theorem PB_Descriptor_IR_format_eq' (desc : PB_Descriptor)
   : forall msg' msg ce,
-    refineEquiv (PB_Message_IR_format_ref' desc msg' msg ce)
-                (PB_Message_IR_format' desc msg' msg ce).
+    refineEquiv (PB_Descriptor_IR_format_ref' desc msg' msg ce)
+                (PB_Descriptor_IR_format' desc msg' msg ce).
 Proof.
   unfold refineEquiv, refine.
-  unfold PB_Message_IR_format_ref', PB_Message_IR_format'. unfold Pick.
+  unfold PB_Descriptor_IR_format_ref', PB_Descriptor_IR_format'. unfold Pick.
   unfold computes_to. simpl.
   intros. split; intros [ir ce'] H; simpl in *. {
     generalize dependent desc.
     generalize dependent ce.
     generalize dependent ce'.
     induction ir as [ir IH] using (well_founded_ind well_founded_lt_b); intros;
-      apply (unroll_LeastFixedPoint_dep PB_Message_IR_format_body_monotone) in H.
+      apply (unroll_LeastFixedPoint_dep PB_Descriptor_IR_format_body_monotone) in H.
     unfold computes_to in H. simpl in H.
     destruct_many;
       try (subst; constructor; eauto; eapply IH; eauto; apply PB_IR_measure_cons_lt || apply PB_IR_measure_embedded_lt).
@@ -1801,7 +1435,7 @@ Proof.
     eapply IH; eauto; apply PB_IR_measure_cons_lt || apply PB_IR_measure_embedded_lt.
     eapply IH; eauto; apply PB_IR_measure_cons_lt || apply PB_IR_measure_embedded_lt.
   } {
-    induction H; intros; apply (unroll_LeastFixedPoint_dep' PB_Message_IR_format_body_monotone);
+    induction H; intros; apply (unroll_LeastFixedPoint_dep' PB_Descriptor_IR_format_body_monotone);
       let rec trial n := match n with
                          | O => try solve [choose_br 0; auto]
                          | S ?n' => try solve [choose_br n; repeat eexists; eauto]; trial n'
@@ -1810,532 +1444,47 @@ Proof.
   }
 Qed.
 
-Theorem PB_Message_IR_format_eq (desc : PB_Message)
+Theorem PB_Descriptor_IR_format_eq (desc : PB_Descriptor)
   : forall msg ce,
-    refineEquiv (PB_Message_IR_format_ref desc msg ce)
-                (PB_Message_IR_format desc msg ce).
+    refineEquiv (PB_Descriptor_IR_format_ref desc msg ce)
+                (PB_Descriptor_IR_format desc msg ce).
 Proof.
-  apply PB_Message_IR_format_eq'.
+  apply PB_Descriptor_IR_format_eq'.
 Qed.
 
-Definition PB_Message_IR_decode_body
-           decode desc (msg : PB_Message_denote desc) ir cd
-  : option (PB_Message_denote desc * PB_IR * CacheDecode) :=
-  match ir with
-  | nil => Some (msg, nil, cd)
-  | Build_PB_IRElm t wty v :: ir' =>
-    match PB_Message_boundedTag desc t with
-    | inl tag =>
-      `(msg1, _, cd1) <- decode desc msg ir' cd;
-        match PB_Message_tagToType tag as x
-              return (PB_Type_denote x -> PB_Message_denote desc) ->
-                     (PB_Type_denote x) ->
-                     _ with
-        | PB_Singular (PB_Primitive pty) =>
-          fun f a =>
-            match PB_WireType_eq_dec wty (PB_PrimitiveType_toWireType pty) with
-            | left pf =>
-              match v with
-              | inl (inl v') =>
-                Some (f (eq_rect _ _ v' _ pf), nil, cd1)
-              | _ => None
-              end
-            | _ => None
-            end
-        | PB_Repeated (PB_Primitive pty) =>
-          fun f a =>
-            match PB_WireType_eq_dec wty (PB_PrimitiveType_toWireType pty) with
-            | left pf =>
-              match v with
-              | inl (inl v') =>
-                Some (f (a ++ [(eq_rect _ _ v' _ pf)]), nil, cd1)
-              | inl (inr l) =>
-                if PB_WireType_eq_dec PB_LengthDelimited (PB_PrimitiveType_toWireType pty) then None
-                else Some (f (a ++ (eq_rect _ (fun wty => list (PB_WireType_denote wty)) l _ pf)), nil, cd1)
-              | _ => None
-              end
-            | _ => None
-            end
-        | PB_Singular (PB_Embedded desc') =>
-          fun f a =>
-            match PB_WireType_eq_dec wty PB_LengthDelimited with
-            | left pf =>
-              match v return _ -> _ with
-              | inr ir2 =>
-                fun decode =>
-                  match a with
-                  | Some msg2 =>
-                    `(msg3, _, cd2) <- decode desc' msg2 ir2 cd1;
-                      Some (f (Some msg3), nil, cd2)
-                  | None =>
-                    `(msg3, _, cd2) <- decode desc' (PB_Message_default desc') ir2 cd1;
-                      Some (f (Some msg3), nil, cd2)
-                  end
-              | _ => fun _ => None
-              end decode
-            | _ => None
-            end
-        | PB_Repeated (PB_Embedded desc') =>
-          fun f a =>
-            match PB_WireType_eq_dec wty PB_LengthDelimited with
-            | left pf =>
-              match v return _ -> _ with
-              | inr ir2 =>
-                fun decode =>
-                  `(msg2, _, cd2) <- decode desc' (PB_Message_default desc') ir2 cd1;
-                    Some (f (a ++ [msg2]), nil, cd2)
-              | _ => fun _ => None
-              end decode
-            | _ => None
-            end
-        end (PB_Message_update msg1 tag) (PB_Message_lookup msg1 tag)
-    | inr tag =>
-      if PB_FieldTag_OK_dec (uindex tag) then
-        match v with
-        | inl (inl _) => decode desc msg ir' cd
-        | _ => None
-        end
-      else None
-    end
-  end.
-
-Definition PB_Message_IR_decode' (desc : PB_Message) (init : PB_Message_denote desc)
-  : DecodeM (PB_Message_denote desc) PB_IR :=
-  FueledFix_dep PB_Message_IR_decode_body desc init.
-
-Definition PB_Message_IR_decode (desc : PB_Message)
-  : DecodeM (PB_Message_denote desc) PB_IR :=
-  PB_Message_IR_decode' desc (PB_Message_default desc).
-
-Lemma PB_Message_IR_Elm_OK (desc : PB_Message)
-      (HP : PB_Message_OK desc)
-      (msg : PB_Message_denote desc) (ir : PB_IR)
+(* The format only produces well-formed IR. *)
+Lemma PB_Descriptor_IR_Elm_OK (desc : PB_Descriptor)
+      (HP : PB_Descriptor_OK desc)
+      (msg : PB_Descriptor_denote desc) (ir : PB_IR)
       (ce ce' : CacheFormat)
-  : PB_Message_IR_format desc msg ce ↝ (ir, ce') ->
+  : PB_Descriptor_IR_format desc msg ce ↝ (ir, ce') ->
     forall elm : PB_IRElm, In elm ir -> PB_IRElm_OK desc elm.
 Proof.
-  intro H. apply (proj1 (PB_Message_IR_format_eq _ _ _)) in H. revert H.
-  unfold PB_Message_IR_format_ref. simpl. unfold computes_to, Pick. simpl.
+  intro H. apply (proj1 (PB_Descriptor_IR_format_eq _ _ _)) in H. revert H.
+  unfold PB_Descriptor_IR_format_ref. simpl. unfold computes_to, Pick. simpl.
   induction 1; intros; try easy;
     match goal with
     | H : In _ _ |- _ => destruct H
     end; auto; subst;
       unfold PB_IRElm_OK;
-      destruct PB_Message_boundedTag eqn:Hb; auto;
+      destruct PB_Descriptor_boundedTag eqn:Hb; auto;
         repeat match goal with
-            | H : PB_Message_boundedTag _ (uindex _) = inl _ |- _ =>
-              exfalso; eapply PB_Message_boundedTag_notl; eauto
-            | H : PB_Message_boundedTag _ (bindex _) = inr _ |- _ =>
-              exfalso; eapply PB_Message_boundedTag_notr; eauto
+            | H : PB_Descriptor_boundedTag _ (uindex _) = inl _ |- _ =>
+              exfalso; eapply PB_Descriptor_boundedTag_notl; eauto
+            | H : PB_Descriptor_boundedTag _ (bindex _) = inr _ |- _ =>
+              exfalso; eapply PB_Descriptor_boundedTag_notr; eauto
             end;
-        try (apply PB_Message_boundedTag_correct in Hb;
+        try (apply PB_Descriptor_boundedTag_correct in Hb;
              apply BoundedTag_inj in Hb; auto; subst;
              rewrite pf; intuition;
-             apply PB_IRElm_OK_equiv in IHPB_IR_refine2; eauto using PB_Message_OK_sub_tagToType).
-  apply PB_Message_boundedTag_correct' in Hb.
+             apply PB_IRElm_OK_equiv in IHPB_IR_transit2; eauto using PB_Descriptor_OK_sub_tagToType).
+  apply PB_Descriptor_boundedTag_correct' in Hb.
   destruct u, t.
   simpl in Hb. subst. auto.
 Qed.
 
-Lemma PB_Message_IR_decode_nil' (desc : PB_Message)
-      (init msg : PB_Message_denote desc) (ir ir' : PB_IR)
-      (cd cd' : CacheDecode)
-  : forall n, FueledFix_dep' PB_Message_IR_decode_body n desc init ir cd = Some (msg, ir', cd') -> ir' = nil.
-Proof.
-  intro. generalize dependent ir. induction n. easy.
-  simpl. unfold PB_Message_IR_decode_body.
-  destruct ir; intros. injections. eauto.
-  destruct p. destruct PB_Message_boundedTag eqn:?. {
-    decode_opt_to_inv.
-    revert H0. generalize (PB_Message_update x b) as update, (PB_Message_lookup x b) as lookup.
-    destruct PB_Message_tagToType eqn:?; destruct p; intros;
-      destruct PB_WireType_eq_dec; repeat destruct s; injections; try easy.
-    destruct lookup; decode_opt_to_inv; easy.
-    destruct PB_WireType_eq_dec; injections; try easy.
-    destruct lookup; decode_opt_to_inv; easy.
-  } {
-    destruct PB_FieldTag_OK_dec eqn:?; try easy.
-    repeat destruct s; try easy.
-    eapply IHn; eauto.
-  }
-Qed.
-
-Lemma PB_Message_IR_decode_nil (desc : PB_Message)
-      (init msg : PB_Message_denote desc) (ir ir' : PB_IR)
-      (cd cd' : CacheDecode)
-  : PB_Message_IR_decode' desc init ir cd = Some (msg, ir', cd') -> ir' = nil.
-Proof.
-  eapply PB_Message_IR_decode_nil'.
-Qed.
-
-Theorem PB_Message_IR_decode_correct' (desc : PB_Message) (init : PB_Message_denote desc)
-        (HP : PB_Message_OK desc)
-        {P : CacheDecode -> Prop}
-        (P_OK : cache_inv_Property P (fun P => forall b cd, P cd -> P (addD cd b)))
-  : CorrectDecoder _
-                   (fun _ => True)
-                   (fun _ ext => ext = mempty)
-                   (PB_Message_IR_format' desc init) (PB_Message_IR_decode' desc init) P.
-Proof.
-  eapply (fix_format_correct_dep _ _ PB_Message_IR_format_body_monotone (fun _ _ => True) (fun _ _ ext => ext = mempty));
-    eauto. intros _. intros.
-  unfold PB_Message_IR_format_body at 1.
-  unfold PB_Message_IR_decode_body at 1.
-  split; intros. {
-    subst ext. unfold computes_to in H5. unfold Pick in H5.
-    destruct_many; subst; simpl in *. {
-      eexists. repeat split; eauto.
-    } {
-      destruct PB_Message_boundedTag eqn:Heq. {
-        eapply H in H4; eauto. 2 : omega. destruct_many.
-        apply PB_Message_boundedTag_correct in Heq.
-        apply BoundedTag_inj in Heq; eauto. subst.
-        rewrite H4. simpl. clear H4.
-
-        generalize (PB_Message_update x0 x1) as update.
-        generalize (PB_Message_lookup x0 x1) as lookup.
-        rewrite x4. intros.
-        destruct PB_WireType_eq_dec; try easy.
-        eexists. repeat split; intros; eauto.
-        repeat f_equal. unfold eq_rect_r. simpl.
-        rewrite <- eq_rect_eq_dec. eauto. apply PB_WireType_eq_dec.
-      } {
-        exfalso. eapply PB_Message_boundedTag_notr; eauto.
-      }
-    } {
-      eapply H in H4; eauto. 2 : omega. destruct_many.
-      destruct PB_Message_boundedTag eqn:Heq. {
-        apply PB_Message_boundedTag_correct in Heq.
-        apply BoundedTag_inj in Heq; eauto. subst.
-        rewrite H4. simpl. clear H4.
-
-        generalize (PB_Message_update x0 x1) as update.
-        generalize (PB_Message_lookup x0 x1) as lookup.
-        rewrite x4. intros.
-        destruct PB_WireType_eq_dec; try easy.
-        eexists. repeat split; intros; eauto.
-        simpl. repeat f_equal. unfold eq_rect_r. simpl.
-        rewrite <- eq_rect_eq_dec. eauto. apply PB_WireType_eq_dec.
-      } {
-        exfalso. eapply PB_Message_boundedTag_notr; eauto.
-      }
-    } {
-      eapply H in H4; eauto. 2 : omega. destruct_many.
-      destruct PB_Message_boundedTag eqn:Heq. {
-        apply PB_Message_boundedTag_correct in Heq.
-        apply BoundedTag_inj in Heq; eauto. subst.
-        rewrite H4. simpl. clear H4.
-
-        generalize (PB_Message_update x0 x1) as update.
-        generalize (PB_Message_lookup x0 x1) as lookup.
-        rewrite x4. intros.
-        destruct PB_WireType_eq_dec; try easy.
-        eexists. repeat split; intros; eauto.
-        repeat f_equal. rewrite <- eq_rect_eq_dec. destruct PB_WireType_eq_dec; auto. congruence.
-        apply PB_WireType_eq_dec.
-      } {
-        exfalso. eapply PB_Message_boundedTag_notr; eauto.
-      }
-    } {
-      eapply H in H4; eauto. 2 : omega. destruct_many.
-      destruct PB_Message_boundedTag eqn:Heq. {
-        exfalso. eapply PB_Message_boundedTag_notl; eauto.
-      } {
-        eexists.
-        destruct PB_FieldTag_OK_dec eqn:?.
-        repeat split; intros; eauto.
-        apply PB_FieldTag_OK_false_iff in Heqb.
-        apply PB_Message_boundedTag_correct' in Heq.
-        destruct u, x0. simpl in Heq. subst. easy.
-      }
-    } {
-      eapply H in H4; eauto. 2 : omega. destruct_many.
-      eapply H in H6; eauto using PB_Message_OK_sub_tagToType.
-      2 : unfold PB_IR_measure, PB_IR_measure'; omega. destruct_many.
-      destruct PB_Message_boundedTag eqn:Heq. {
-        apply PB_Message_boundedTag_correct in Heq.
-        apply BoundedTag_inj in Heq; eauto. subst.
-        rewrite H4. simpl. clear H4.
-
-        revert H5.
-        generalize (PB_Message_update x0 x1) as update.
-        generalize (PB_Message_lookup x0 x1) as lookup.
-        rewrite x5. intros.
-        match goal with
-        | H : ?a = None |-
-          context [match ?b with _ => _ end] => replace b with a; [rewrite H |]
-        end.
-        rewrite app_nil_r in H6. rewrite H6. clear H6. simpl.
-        eexists. repeat split; intros; eauto.
-        simpl. reflexivity.
-      } {
-        exfalso. eapply PB_Message_boundedTag_notr; eauto.
-      }
-    } {
-      eapply H in H4; eauto. 2 : omega. destruct_many.
-      eapply H in H6; eauto using PB_Message_OK_sub_tagToType.
-      2 : unfold PB_IR_measure, PB_IR_measure'; omega. destruct_many.
-      destruct PB_Message_boundedTag eqn:Heq. {
-        apply PB_Message_boundedTag_correct in Heq.
-        apply BoundedTag_inj in Heq; eauto. subst.
-        rewrite H4. simpl. clear H4.
-
-        revert H5.
-        generalize (PB_Message_update x0 x1) as update.
-        generalize (PB_Message_lookup x0 x1) as lookup.
-        rewrite x6. intros.
-        match goal with
-        | H : ?a = Some _ |-
-          context [match ?b with _ => _ end] => replace b with a; [rewrite H |]
-        end.
-        rewrite app_nil_r in H6. rewrite H6. clear H6. simpl.
-        eexists. repeat split; intros; eauto.
-        simpl. reflexivity.
-      } {
-        exfalso. eapply PB_Message_boundedTag_notr; eauto.
-      }
-    } {
-      eapply H in H4; eauto. 2 : omega. destruct_many.
-      eapply H in H5; eauto using PB_Message_OK_sub_tagToType.
-      2 : unfold PB_IR_measure, PB_IR_measure'; omega. destruct_many.
-      destruct PB_Message_boundedTag eqn:Heq. {
-        apply PB_Message_boundedTag_correct in Heq.
-        apply BoundedTag_inj in Heq; eauto. subst.
-        rewrite H4. simpl. clear H4.
-
-        generalize (PB_Message_update x0 x1) as update.
-        generalize (PB_Message_lookup x0 x1) as lookup.
-        rewrite x5. intros.
-        rewrite app_nil_r in H5. rewrite H5. clear H5. simpl.
-        eexists. repeat split; intros; eauto.
-      } {
-        exfalso. eapply PB_Message_boundedTag_notr; eauto.
-      }
-    }
-  } {
-    unfold computes_to in *. unfold Pick in *.
-    destruct b. {
-      injections. split; auto.
-      exists [], env. repeat split; eauto.
-    } {
-      destruct p.
-      destruct PB_Message_boundedTag eqn:Heq; simpl in *. {
-        decode_opt_to_inv.
-        pose proof H4 as Hnil. apply PB_Message_IR_decode_nil' in Hnil. subst.
-        (* :TODO: better solution? ? ?@ *)
-        assert (exists (msg : PB_Message_denote d) (t : BoundedTag d) pf,
-                   PB_Message_lookup x b0 = (eq_rect _ _ (PB_Message_lookup msg t) _ pf) /\
-                   x = msg /\ b0 = t /\ forall pf', pf = pf') as L1. {
-          eexists _, _, eq_refl. intuition eauto.
-          apply UIP_dec. apply PB_Type_eq_dec.
-        }
-        assert (forall a1,
-                   exists (msg : PB_Message_denote d) (t : BoundedTag d) pf,
-                     PB_Message_update x b0 a1 = PB_Message_update msg t (eq_rect_r _ a1 pf) /\
-                     x = msg /\ b0 = t /\ forall pf', pf = pf') as L2. {
-          intros. eexists _, _, eq_refl. intuition eauto.
-          apply UIP_dec. apply PB_Type_eq_dec.
-        }
-        revert L1 L2 H5.
-        generalize (PB_Message_update x b0) as update.
-        generalize (PB_Message_lookup x b0) as lookup.
-        simpl in *. intros.
-
-        destruct PB_Message_tagToType eqn:?; destruct p; intros. {
-          apply PB_Message_boundedTag_correct in Heq. subst.
-          destruct PB_WireType_eq_dec; repeat destruct s; injections; try easy.
-          eapply H in H4; eauto using PB_IR_measure_cons_lt. 2 : omega. intuition.
-          destruct_many. rewrite app_nil_r in *. subst.
-          eexists _, _. repeat split; eauto.
-          2 : rewrite app_nil_r; reflexivity.
-          choose_br 1.
-          match goal with
-          | |- context [update ?a] => specialize (L2 a)
-          end. destruct_many. subst.
-          repeat eexists; eauto.
-        } {
-          apply PB_Message_boundedTag_correct in Heq. subst.
-          destruct PB_WireType_eq_dec; repeat destruct s; injections; try easy.
-          destruct lookup eqn:?. {
-            decode_opt_to_inv. subst.
-            pose proof H5 as Hnil. apply PB_Message_IR_decode_nil' in Hnil. subst.
-            eapply H in H4; eauto using PB_IR_measure_cons_lt. 2 : omega. destruct_many.
-            eapply H in H5; eauto using PB_IR_measure_embedded_lt, PB_Message_OK_sub_tagToType.
-            2 : unfold PB_IR_measure, PB_IR_measure'; omega. destruct_many.
-            intuition. simpl in *. rewrite app_nil_r in *. subst.
-            eexists _, _. repeat split; eauto.
-            2 : rewrite app_nil_r; reflexivity.
-            choose_br 6.
-            match goal with
-            | |- context [update ?a] => specialize (L2 a)
-            end. destruct_many. subst.
-            repeat eexists; eauto.
-            match goal with
-            | H : update ?a = ?b |- _ => rewrite H
-            end. repeat f_equal. eauto.
-          } {
-            decode_opt_to_inv. subst.
-            pose proof H5 as Hnil. apply PB_Message_IR_decode_nil' in Hnil. subst.
-            eapply H in H4; eauto using PB_IR_measure_cons_lt. 2 : omega. destruct_many.
-            eapply H in H5; eauto using PB_IR_measure_embedded_lt, PB_Message_OK_sub_tagToType.
-            2 : unfold PB_IR_measure, PB_IR_measure'; omega. destruct_many.
-            intuition. simpl in *. rewrite app_nil_r in *. subst.
-            eexists _, _. repeat split; eauto.
-            2 : rewrite app_nil_r; reflexivity.
-            choose_br 5.
-            match goal with
-            | |- context [update ?a] => specialize (L2 a)
-            end. destruct_many. subst.
-            repeat eexists; eauto.
-            match goal with
-            | H : update ?a = ?b |- _ => rewrite H
-            end. repeat f_equal. eauto.
-          }
-        } {
-          apply PB_Message_boundedTag_correct in Heq. subst.
-          destruct PB_WireType_eq_dec; repeat destruct s; injections; try easy. {
-            eapply H in H4; eauto using PB_IR_measure_cons_lt. 2 : omega. destruct_many.
-            intuition. simpl in *. rewrite app_nil_r in *. subst.
-            eexists _, _. repeat split; eauto.
-            2 : rewrite app_nil_r; reflexivity.
-            choose_br 2.
-            match goal with
-            | |- context [update ?a] => specialize (L2 a)
-            end. destruct_many. subst.
-            repeat eexists; eauto.
-            match goal with
-            | H : update ?a = ?b |- _ => rewrite H
-            end. repeat f_equal. eauto.
-          } {
-            destruct PB_WireType_eq_dec; [easy |]. injections.
-            eapply H in H4; eauto using PB_IR_measure_cons_lt. 2 : omega. destruct_many.
-            intuition. simpl in *. rewrite app_nil_r in *. subst.
-            eexists _, _. repeat split; eauto.
-            2 : rewrite app_nil_r; reflexivity.
-            choose_br 3.
-            match goal with
-            | |- context [update ?a] => specialize (L2 a)
-            end. destruct_many. subst.
-            repeat eexists; eauto.
-            match goal with
-            | H : update ?a = ?b |- _ => rewrite H
-            end. repeat f_equal. eauto.
-          }
-        } {
-          apply PB_Message_boundedTag_correct in Heq. subst.
-          destruct PB_WireType_eq_dec; repeat destruct s; injections; try easy.
-          decode_opt_to_inv. subst.
-          pose proof H5 as Hnil. apply PB_Message_IR_decode_nil' in Hnil. subst.
-          eapply H in H4; eauto using PB_IR_measure_cons_lt. 2 : omega. destruct_many.
-          eapply H in H5; eauto using PB_IR_measure_embedded_lt, PB_Message_OK_sub_tagToType.
-          2 : unfold PB_IR_measure, PB_IR_measure'; omega. destruct_many.
-          intuition. simpl in *. rewrite app_nil_r in *. subst.
-          eexists _, _. repeat split; eauto.
-          2 : rewrite app_nil_r; reflexivity.
-          choose_br 7.
-          match goal with
-          | |- context [update ?a] => specialize (L2 a)
-          end. destruct_many. subst.
-          repeat eexists; eauto.
-          match goal with
-          | H : update ?a = ?b |- _ => rewrite H
-          end. repeat f_equal. eauto.
-        }
-      } {
-        apply PB_Message_boundedTag_correct' in Heq. subst.
-        destruct PB_FieldTag_OK_dec eqn:?; try easy.
-        repeat destruct s; try easy.
-        pose proof H4 as Hnil. apply PB_Message_IR_decode_nil' in Hnil. subst.
-        eapply H in H4; eauto using PB_IR_measure_cons_lt. 2 : omega. destruct_many.
-        intuition. simpl in *. rewrite app_nil_r in *. subst.
-        eexists _, _. repeat split; eauto.
-        2 : rewrite app_nil_r; reflexivity.
-        choose_br 4.
-        repeat eexists; eauto. apply PB_FieldTag_OK_true_iff in Heqb0. auto.
-      }
-    }
-  }
-
-  intros. unfold PB_Message_IR_decode_body in H0.  unfold PB_Message_IR_decode_body at 1.
-  destruct b; eauto.
-  destruct p. destruct PB_Message_boundedTag.
-  decode_opt_to_inv. apply H in H0. rewrite H0. simpl.
-  revert H1.
-  generalize (PB_Message_update x b0) as update. generalize (PB_Message_lookup x b0) as lookup.
-  destruct PB_Message_tagToType; intros;
-    destruct p; destruct PB_WireType_eq_dec; destruct s; eauto;
-      destruct lookup; decode_opt_to_inv; apply H in H1; rewrite H1; eauto.
-  destruct PB_FieldTag_OK_dec eqn:?; try easy.
-  destruct s; eauto. destruct s; eauto.
-
-  Grab Existential Variables. all : auto.
-Qed.
-
-Theorem PB_Message_IR_decode_correct (desc : PB_Message)
-        (HP : PB_Message_OK desc)
-        {P : CacheDecode -> Prop}
-        (P_OK : cache_inv_Property P (fun P => forall b cd, P cd -> P (addD cd b)))
-  : CorrectDecoder _
-                   (fun _ => True)
-                   (fun _ ext => ext = mempty)
-                   (PB_Message_IR_format desc) (PB_Message_IR_decode desc) P.
-Proof.
-  apply PB_Message_IR_decode_correct'; eauto.
-Qed.
-
-Definition PB_Message_format (desc : PB_Message)
-  : FormatM (PB_Message_denote desc) ByteString :=
+(* The end-to-end format is just a composition of the formats of layers. *)
+Definition PB_Descriptor_format (desc : PB_Descriptor)
+  : FormatM (PB_Descriptor_denote desc) ByteString :=
   (fun msg ce =>
-     `(ir, _) <- PB_Message_IR_format desc msg ce; SizedList_format PB_IRElm_format (rev ir) ce)%comp.
-
-Definition PB_Message_decode (desc : PB_Message)
-  : DecodeM (PB_Message_denote desc) ByteString :=
-  fun b cd =>
-    `(ir, b', cd') <- SizedList_decode (PB_IRElm_decode desc) (bin_measure b) b cd;
-      `(msg, _, _) <- PB_Message_IR_decode desc (rev ir) cd;
-      Some (msg, b', cd').
-
-Theorem PB_Message_decode_correct (desc : PB_Message)
-        (HP : PB_Message_OK desc)
-        {P : CacheDecode -> Prop}
-        (P_OK : cache_inv_Property P (fun P => forall b cd, P cd -> P (addD cd b)))
-  : CorrectDecoder _
-                   (fun _ => True)
-                   (fun _ ext => ext = mempty)
-                   (PB_Message_format desc) (PB_Message_decode desc) P.
-Proof.
-  unfold PB_Message_format, PB_Message_decode.
-  split; intros. {
-    subst.
-    computes_to_inv2.
-    pose proof H2.
-    eapply (PB_Message_IR_decode_correct desc HP P_OK) in H2; eauto. destruct_many.
-    clear H3 H4.
-    eapply (SizedList_decode_correct _ _ _ _ P) in H2';
-      eauto using PB_IRElm_decode_correct, PB_IRElm_format_sz_eq, PB_IRElm_format_some.
-    3 : apply SizedList_predicate_rest_True.
-    2 : {
-      split. intros; eapply (SizedList_format_sz_eq _ PB_IRElm_format_sz_eq); eauto.
-      intros. rewrite <- in_rev in *.
-      eapply PB_Message_IR_Elm_OK; eauto.
-    }
-    destruct_many.
-    eexists. repeat split; eauto.
-    rewrite @mempty_right in *.
-    rewrite H3. simpl. rewrite rev_involutive.
-    rewrite H2. eauto.
-  } {
-    decode_opt_to_inv. subst.
-    eapply (SizedList_decode_correct _ _ _ _ P) in H1;
-      eauto using PB_IRElm_decode_correct, PB_IRElm_format_sz_eq, PB_IRElm_format_some.
-    destruct_many.
-    pose proof H2 as Hnil. apply PB_Message_IR_decode_nil in Hnil. subst.
-    eapply (PB_Message_IR_decode_correct desc HP P_OK) in H2; eauto. destruct_many.
-    subst. split; eauto. eexists _, _. repeat split; eauto.
-    computes_to_econstructor; eauto. simpl.
-    rewrite @mempty_right in *. subst.
-    rewrite rev_involutive. eauto.
-  }
-Qed.
-
-Print Assumptions PB_Message_decode_correct.
+     `(ir, _) <- PB_Descriptor_IR_format desc msg ce; SizedList_format PB_IRElm_format (rev ir) ce)%comp.
