src/Protobuf/conformance/ProtobufConformance.v
@@ -4,65 +4,65 @@ Require Import
 
 Open Scope Protobuf_scope.
 
-Definition NestedMessage : PB_Message :=
-  [(PB_Singular (PB_Primitive PB_int32), "a", 1)].
+Definition NestedMessage : PB_Descriptor :=
+  [(PB_Singular (PB_Base PB_int32), "a", 1)].
 
-Definition ForeignMessage : PB_Message :=
-  [(PB_Singular (PB_Primitive PB_int32), "c", 1)].
+Definition ForeignMessage : PB_Descriptor :=
+  [(PB_Singular (PB_Base PB_int32), "c", 1)].
 
 (* We use compatible types for high-level types that we don't support yet. *)
-Definition TestAllTypesProto3 : PB_Message :=
-  [(PB_Singular (PB_Primitive PB_int32), "optional_int32", 1);
-   ((PB_Singular (PB_Primitive PB_int64)), "optional_int64", 2);
-   (PB_Singular (PB_Primitive PB_int32), "optional_uint32", 3);
-   (PB_Singular (PB_Primitive PB_int64), "optional_uint64", 4);
-   (PB_Singular (PB_Primitive PB_int32), "optional_sint32", 5);
-   (PB_Singular (PB_Primitive PB_int64), "optional_sint64", 6);
-   (PB_Singular (PB_Primitive PB_fixed32), "optional_fixed32", 7);
-   (PB_Singular (PB_Primitive PB_fixed64), "optional_fixed64", 8);
-   (PB_Singular (PB_Primitive PB_fixed32), "optional_sfixed32", 9);
-   (PB_Singular (PB_Primitive PB_fixed64), "optional_sfixed64", 10);
-   (PB_Singular (PB_Primitive PB_fixed32), "optional_float", 11);
-   (PB_Singular (PB_Primitive PB_fixed64), "optional_double", 12);
-   (PB_Singular (PB_Primitive PB_int32), "optional_bool", 13);
-   (PB_Singular (PB_Primitive PB_string), "optional_string", 14);
-   (PB_Singular (PB_Primitive PB_string), "optional_bytes", 15);
+Definition TestAllTypesProto3 : PB_Descriptor :=
+  [(PB_Singular (PB_Base PB_int32), "optional_int32", 1);
+   ((PB_Singular (PB_Base PB_int64)), "optional_int64", 2);
+   (PB_Singular (PB_Base PB_int32), "optional_uint32", 3);
+   (PB_Singular (PB_Base PB_int64), "optional_uint64", 4);
+   (PB_Singular (PB_Base PB_int32), "optional_sint32", 5);
+   (PB_Singular (PB_Base PB_int64), "optional_sint64", 6);
+   (PB_Singular (PB_Base PB_fixed32), "optional_fixed32", 7);
+   (PB_Singular (PB_Base PB_fixed64), "optional_fixed64", 8);
+   (PB_Singular (PB_Base PB_fixed32), "optional_sfixed32", 9);
+   (PB_Singular (PB_Base PB_fixed64), "optional_sfixed64", 10);
+   (PB_Singular (PB_Base PB_fixed32), "optional_float", 11);
+   (PB_Singular (PB_Base PB_fixed64), "optional_double", 12);
+   (PB_Singular (PB_Base PB_int32), "optional_bool", 13);
+   (PB_Singular (PB_Base PB_string), "optional_string", 14);
+   (PB_Singular (PB_Base PB_string), "optional_bytes", 15);
 
    (PB_Singular (PB_Embedded NestedMessage), "optional_nested_message", 18);
    (PB_Singular (PB_Embedded ForeignMessage), "optional_foreign_message", 19);
-   (PB_Singular (PB_Primitive PB_int32), "optional_nested_enum", 21);
-   (PB_Singular (PB_Primitive PB_int32), "optional_foreign_enum", 22);
+   (PB_Singular (PB_Base PB_int32), "optional_nested_enum", 21);
+   (PB_Singular (PB_Base PB_int32), "optional_foreign_enum", 22);
 
-   (PB_Singular (PB_Primitive PB_string), "optional_string_piece", 24);
-   (PB_Singular (PB_Primitive PB_string), "optional_cord", 25);
+   (PB_Singular (PB_Base PB_string), "optional_string_piece", 24);
+   (PB_Singular (PB_Base PB_string), "optional_cord", 25);
 
-   (PB_Repeated (PB_Primitive PB_int32), "repeated_int32", 31);
-   (PB_Repeated (PB_Primitive PB_int64), "repeated_int64", 32);
-   (PB_Repeated (PB_Primitive PB_int32), "repeated_uint32", 33);
-   (PB_Repeated (PB_Primitive PB_int64), "repeated_uint64", 34);
-   (PB_Repeated (PB_Primitive PB_int32), "repeated_sint32", 35);
-   (PB_Repeated (PB_Primitive PB_int64), "repeated_sint64", 36);
-   (PB_Repeated (PB_Primitive PB_fixed32), "repeated_fixed32", 37);
-   (PB_Repeated (PB_Primitive PB_fixed64), "repeated_fixed64", 38);
-   (PB_Repeated (PB_Primitive PB_fixed32), "repeated_sfixed32", 39);
-   (PB_Repeated (PB_Primitive PB_fixed64), "repeated_sfixed64", 40);
-   (PB_Repeated (PB_Primitive PB_fixed32), "repeated_float", 41);
-   (PB_Repeated (PB_Primitive PB_fixed64), "repeated_double", 42);
-   (PB_Repeated (PB_Primitive PB_int32), "repeated_bool", 43);
-   (PB_Repeated (PB_Primitive PB_string), "repeated_string", 44);
-   (PB_Repeated (PB_Primitive PB_string), "repeated_bytes", 45);
+   (PB_Repeated (PB_Base PB_int32), "repeated_int32", 31);
+   (PB_Repeated (PB_Base PB_int64), "repeated_int64", 32);
+   (PB_Repeated (PB_Base PB_int32), "repeated_uint32", 33);
+   (PB_Repeated (PB_Base PB_int64), "repeated_uint64", 34);
+   (PB_Repeated (PB_Base PB_int32), "repeated_sint32", 35);
+   (PB_Repeated (PB_Base PB_int64), "repeated_sint64", 36);
+   (PB_Repeated (PB_Base PB_fixed32), "repeated_fixed32", 37);
+   (PB_Repeated (PB_Base PB_fixed64), "repeated_fixed64", 38);
+   (PB_Repeated (PB_Base PB_fixed32), "repeated_sfixed32", 39);
+   (PB_Repeated (PB_Base PB_fixed64), "repeated_sfixed64", 40);
+   (PB_Repeated (PB_Base PB_fixed32), "repeated_float", 41);
+   (PB_Repeated (PB_Base PB_fixed64), "repeated_double", 42);
+   (PB_Repeated (PB_Base PB_int32), "repeated_bool", 43);
+   (PB_Repeated (PB_Base PB_string), "repeated_string", 44);
+   (PB_Repeated (PB_Base PB_string), "repeated_bytes", 45);
 
    (PB_Repeated (PB_Embedded NestedMessage), "repeated_nested_message", 48);
    (PB_Repeated (PB_Embedded ForeignMessage), "repeated_foreign_message", 49);
-   (PB_Repeated (PB_Primitive PB_int32), "repeated_nested_enum", 51);
-   (PB_Repeated (PB_Primitive PB_int32), "repeated_foreign_enum", 52);
+   (PB_Repeated (PB_Base PB_int32), "repeated_nested_enum", 51);
+   (PB_Repeated (PB_Base PB_int32), "repeated_foreign_enum", 52);
 
-   (PB_Repeated (PB_Primitive PB_string), "repeated_string_piece", 54);
-   (PB_Repeated (PB_Primitive PB_string), "repeated_cord", 55)].
+   (PB_Repeated (PB_Base PB_string), "repeated_string_piece", 54);
+   (PB_Repeated (PB_Base PB_string), "repeated_cord", 55)].
 
-Definition testall_encode := PB_Message_encode_impl TestAllTypesProto3.
+Definition testall_encode := PB_Descriptor_encode_impl TestAllTypesProto3.
 
-Definition testall_decode := PB_Message_decode_impl TestAllTypesProto3.
+Definition testall_decode := PB_Descriptor_decode_impl TestAllTypesProto3.
 
 Extraction "testall"
            Vector.to_list Vector.of_list
