src/Protobuf/examples/ProtobufExample.v
@@ -3,27 +3,27 @@ Require Import
 
 Open Scope Protobuf_scope.
 
-Definition Timestamp : PB_Message :=
-  [(PB_Singular (PB_Primitive PB_int64), "seconds", 1);
-   (PB_Singular (PB_Primitive PB_int32), "nanos", 2)].
+Definition Timestamp : PB_Descriptor :=
+  [(PB_Singular (PB_Base PB_int64), "seconds", 1);
+   (PB_Singular (PB_Base PB_int32), "nanos", 2)].
 
-Definition PhoneNumber : PB_Message :=
-  [(PB_Singular (PB_Primitive PB_string), "number", 1);
-   (PB_Singular (PB_Primitive PB_int32), "type", 2)].
+Definition PhoneNumber : PB_Descriptor :=
+  [(PB_Singular (PB_Base PB_string), "number", 1);
+   (PB_Singular (PB_Base PB_int32), "type", 2)].
 
-Definition Person : PB_Message :=
-  [(PB_Singular (PB_Primitive PB_string), "name", 1);
-   (PB_Singular (PB_Primitive PB_int32), "id", 2);
-   (PB_Singular (PB_Primitive PB_string), "email", 3);
+Definition Person : PB_Descriptor :=
+  [(PB_Singular (PB_Base PB_string), "name", 1);
+   (PB_Singular (PB_Base PB_int32), "id", 2);
+   (PB_Singular (PB_Base PB_string), "email", 3);
    (PB_Repeated (PB_Embedded PhoneNumber), "phones", 4);
    (PB_Singular (PB_Embedded Timestamp), "last_updated", 5)].
 
-Definition AddressBook : PB_Message :=
+Definition AddressBook : PB_Descriptor :=
   [(PB_Repeated (PB_Embedded Person), "people", 1)].
 
-Definition AddressBook_encode := PB_Message_encode_impl AddressBook.
+Definition AddressBook_encode := PB_Descriptor_encode_impl AddressBook.
 
-Definition AddressBook_decode := PB_Message_decode_impl AddressBook.
+Definition AddressBook_decode := PB_Descriptor_decode_impl AddressBook.
 
 (* Boilerplate for easier access to the message in the extracted code. *)
 Require Import
@@ -34,29 +34,29 @@ Require Import
 Open Scope Tuple_scope.
 
 Definition Timestamp_construct
-           (seconds : N) (nanos : N) : PB_Message_denote Timestamp :=
+           (seconds : N) (nanos : N) : PB_Descriptor_denote Timestamp :=
   <"seconds" :: seconds,
    "nanos" :: nanos>.
 
 Definition Timestamp_destruct {A}
            (f : N -> N -> A)
-           (msg : PB_Message_denote Timestamp) :=
+           (msg : PB_Descriptor_denote Timestamp) :=
   f msg!"seconds" msg!"nanos".
 
 Definition PhoneNumber_construct
-           (number : list char) (type : N) : PB_Message_denote PhoneNumber :=
+           (number : list char) (type : N) : PB_Descriptor_denote PhoneNumber :=
   <"number" :: number,
    "type" :: type>.
 
 Definition PhoneNumber_destruct {A}
            (f : list char -> N -> A)
-           (msg : PB_Message_denote PhoneNumber) :=
+           (msg : PB_Descriptor_denote PhoneNumber) :=
   f msg!"number" msg!"type".
 
 Definition Person_construct
            (name : list char) (id : N) (email : list char)
-           (phones : list (PB_Message_denote PhoneNumber))
-           (last_updated : option (PB_Message_denote Timestamp)) : PB_Message_denote Person :=
+           (phones : list (PB_Descriptor_denote PhoneNumber))
+           (last_updated : option (PB_Descriptor_denote Timestamp)) : PB_Descriptor_denote Person :=
   <"name" :: name,
    "id" :: id,
    "email" :: email,
@@ -65,19 +65,19 @@ Definition Person_construct
 
 Definition Person_destruct {A}
            (f : list char -> N -> list char ->
-                list (PB_Message_denote PhoneNumber) ->
-                option (PB_Message_denote Timestamp) -> A)
-           (msg : PB_Message_denote Person)
+                list (PB_Descriptor_denote PhoneNumber) ->
+                option (PB_Descriptor_denote Timestamp) -> A)
+           (msg : PB_Descriptor_denote Person)
            : A :=
   f msg!"name" msg!"id" msg!"email" msg!"phones" msg!"last_updated".
 
 Definition AddressBook_construct
-           (people : list (PB_Message_denote Person)) : PB_Message_denote AddressBook :=
+           (people : list (PB_Descriptor_denote Person)) : PB_Descriptor_denote AddressBook :=
   <"people" :: people>.
 
 Definition AddressBook_destruct {A}
-           (f : list (PB_Message_denote Person) -> A)
-           (msg : PB_Message_denote AddressBook) :=
+           (f : list (PB_Descriptor_denote Person) -> A)
+           (msg : PB_Descriptor_denote AddressBook) :=
   f msg!"people".
 
 Extraction "addressbook"
